<?xml version="1.0" encoding="UTF-8"?>
<rdf:RDF xmlns:rdf="http://www.w3.org/1999/02/22-rdf-syntax-ns#">
  <skos:ConceptScheme xmlns:skos="http://www.w3.org/2004/02/skos/core#" rdf:about="http://inspire.ec.europa.eu/metadata-codelist/SpatialDataServiceCategory">
    <dc:title xmlns:dc="http://purl.org/dc/elements/1.1/" xml:lang="en">Classification of spatial data services</dc:title>
    <dc:description xmlns:dc="http://purl.org/dc/elements/1.1/" xml:lang="en">The keywords are based on the geographic services taxonomy of EN ISO 19119. This taxonomy is organised in categories, the subcategories defining the value domain of the classification of spatial data services.</dc:description>
    <dc:title xmlns:dc="http://purl.org/dc/elements/1.1/" xml:lang="es">Clasificación de los servicios de datos espaciales</dc:title>
    <dc:description xmlns:dc="http://purl.org/dc/elements/1.1/" xml:lang="es">Las palabras clave se basan en la taxonomía de servicios geográficos de la norma EN ISO 19119. Esta taxonomía se organiza en categorías, divididas en subcategorías que definen el dominio de valores de la clasificación de los servicios de datos espaciales.</dc:description>
    <dc:title xmlns:dc="http://purl.org/dc/elements/1.1/" xml:lang="fr">Classification des services de données géographiques</dc:title>
    <dc:description xmlns:dc="http://purl.org/dc/elements/1.1/" xml:lang="fr">Les mots clés sont fondés sur la taxonomie des services géographiques de la norme EN ISO 19119. Cette taxonomie est organisée en catégories, elles-mêmes divisées en sous-catégories qui déterminent le domaine de valeur de la classification des services de données géographiques.</dc:description>
    <dc:title xmlns:dc="http://purl.org/dc/elements/1.1/" xml:lang="pt">Classificação dos serviços de dados geográficos</dc:title>
    <dc:description xmlns:dc="http://purl.org/dc/elements/1.1/" xml:lang="pt">As palavras-chave têm por base a taxonomia de serviços geográficos da norma EN ISO 19119. Esta taxonomia está organizada em categorias, com as subcategorias a definir o domínio de valores da classificação de serviços de dados geográficos.</dc:description>
    <dcterms:issued xmlns:dcterms="http://purl.org/dc/terms/">2019-09-30T12:06:20</dcterms:issued>
    <dcterms:modified xmlns:dcterms="http://purl.org/dc/terms/">2019-09-30T12:06:20</dcterms:modified>
    <skos:hasTopConcept rdf:resource="http://inspire.ec.europa.eu/metadata-codelist/SpatialDataServiceCategory/humanInteractionService" />
    <skos:hasTopConcept rdf:resource="http://inspire.ec.europa.eu/metadata-codelist/SpatialDataServiceCategory/infoManagementService" />
    <skos:hasTopConcept rdf:resource="http://inspire.ec.europa.eu/metadata-codelist/SpatialDataServiceCategory/taskManagementService" />
    <skos:hasTopConcept rdf:resource="http://inspire.ec.europa.eu/metadata-codelist/SpatialDataServiceCategory/spatialProcessingService" />
    <skos:hasTopConcept rdf:resource="http://inspire.ec.europa.eu/metadata-codelist/SpatialDataServiceCategory/thematicProcessingService" />
    <skos:hasTopConcept rdf:resource="http://inspire.ec.europa.eu/metadata-codelist/SpatialDataServiceCategory/temporalProcessingService" />
    <skos:hasTopConcept rdf:resource="http://inspire.ec.europa.eu/metadata-codelist/SpatialDataServiceCategory/metadataProcessingService" />
    <skos:hasTopConcept rdf:resource="http://inspire.ec.europa.eu/metadata-codelist/SpatialDataServiceCategory/comService" />
  </skos:ConceptScheme>
  <skos:Concept xmlns:skos="http://www.w3.org/2004/02/skos/core#" rdf:about="http://inspire.ec.europa.eu/metadata-codelist/SpatialDataServiceCategory/humanInteractionService">
    <skos:prefLabel xml:lang="en">Geographic human interaction services</skos:prefLabel>
    <skos:prefLabel xml:lang="es">Servicios geográficos de interacción humana</skos:prefLabel>
    <skos:prefLabel xml:lang="fr">Services géographiques avec interaction humaine</skos:prefLabel>
    <skos:prefLabel xml:lang="pt">Serviços geográficos com interacção humana</skos:prefLabel>
    <skos:inScheme rdf:resource="http://inspire.ec.europa.eu/metadata-codelist/SpatialDataServiceCategory" />
    <skos:narrower rdf:resource="http://inspire.ec.europa.eu/metadata-codelist/SpatialDataServiceCategory/humanCatalogueViewer" />
    <skos:narrower rdf:resource="http://inspire.ec.europa.eu/metadata-codelist/SpatialDataServiceCategory/humanGeographicViewer" />
    <skos:narrower rdf:resource="http://inspire.ec.europa.eu/metadata-codelist/SpatialDataServiceCategory/humanGeographicSpreadsheetViewer" />
    <skos:narrower rdf:resource="http://inspire.ec.europa.eu/metadata-codelist/SpatialDataServiceCategory/humanServiceEditor" />
    <skos:narrower rdf:resource="http://inspire.ec.europa.eu/metadata-codelist/SpatialDataServiceCategory/humanChainDefinitionEditor" />
    <skos:narrower rdf:resource="http://inspire.ec.europa.eu/metadata-codelist/SpatialDataServiceCategory/humanWorkflowEnactmentManager" />
    <skos:narrower rdf:resource="http://inspire.ec.europa.eu/metadata-codelist/SpatialDataServiceCategory/humanGeographicFeatureEditor" />
    <skos:narrower rdf:resource="http://inspire.ec.europa.eu/metadata-codelist/SpatialDataServiceCategory/humanGeographicSymbolEditor" />
    <skos:narrower rdf:resource="http://inspire.ec.europa.eu/metadata-codelist/SpatialDataServiceCategory/humanFeatureGeneralizationEditor" />
    <skos:narrower rdf:resource="http://inspire.ec.europa.eu/metadata-codelist/SpatialDataServiceCategory/humanGeographicDataStructureViewer" />
  </skos:Concept>
  <skos:Concept xmlns:skos="http://www.w3.org/2004/02/skos/core#" rdf:about="http://inspire.ec.europa.eu/metadata-codelist/SpatialDataServiceCategory/humanCatalogueViewer">
    <skos:prefLabel xml:lang="en">Catalogue viewer</skos:prefLabel>
    <skos:scopeNote xml:lang="en">Client service that allows a user to interact with a catalogue to locate, browse, and manage metadata about geographic data or geographic services.</skos:scopeNote>
    <skos:prefLabel xml:lang="es">Visor de catálogos</skos:prefLabel>
    <skos:scopeNote xml:lang="es">Servicio cliente que permite al usuario interactuar con un catálogo para localizar, navegar y gestionar metadatos sobre datos geográficos o servicios geográficos.</skos:scopeNote>
    <skos:prefLabel xml:lang="fr">Visualiseur de catalogue</skos:prefLabel>
    <skos:scopeNote xml:lang="fr">Service client permettant l’interaction de l’utilisateur avec un catalogue afin de localiser, parcourir et gérer des métadonnées concernant des données ou des services géographiques.</skos:scopeNote>
    <skos:prefLabel xml:lang="pt">Visualizador de catálogo</skos:prefLabel>
    <skos:scopeNote xml:lang="pt">Serviço cliente que permite ao utilizador interagir com um catálogo para localizar, navegar e gerir metadados sobre dados geográficos ou serviços geográficos.</skos:scopeNote>
    <skos:inScheme rdf:resource="http://inspire.ec.europa.eu/metadata-codelist/SpatialDataServiceCategory" />
    <skos:broader rdf:resource="http://inspire.ec.europa.eu/metadata-codelist/SpatialDataServiceCategory/humanInteractionService" />
  </skos:Concept>
  <skos:Concept xmlns:skos="http://www.w3.org/2004/02/skos/core#" rdf:about="http://inspire.ec.europa.eu/metadata-codelist/SpatialDataServiceCategory/humanGeographicViewer">
    <skos:prefLabel xml:lang="en">Geographic viewer</skos:prefLabel>
    <skos:scopeNote xml:lang="en">Client service that allows a user to view one or more feature collections or coverages.</skos:scopeNote>
    <skos:prefLabel xml:lang="es">Visor geográfico</skos:prefLabel>
    <skos:scopeNote xml:lang="es">Servicio cliente que permite al usuario visualizar una o más colecciones de fenómenos o coberturas.</skos:scopeNote>
    <skos:prefLabel xml:lang="fr">Service de visualisation géographique</skos:prefLabel>
    <skos:scopeNote xml:lang="fr">Service client permettant à l’utilisateur de visualiser une ou plusieurs compilations d’éléments ou couvertures.</skos:scopeNote>
    <skos:prefLabel xml:lang="pt">Visualizador geográfico</skos:prefLabel>
    <skos:scopeNote xml:lang="pt">Serviço cliente que permite ao utilizador visualizar uma ou mais colecções de elementos geográficos ou coberturas.</skos:scopeNote>
    <skos:inScheme rdf:resource="http://inspire.ec.europa.eu/metadata-codelist/SpatialDataServiceCategory" />
    <skos:broader rdf:resource="http://inspire.ec.europa.eu/metadata-codelist/SpatialDataServiceCategory/humanInteractionService" />
  </skos:Concept>
  <skos:Concept xmlns:skos="http://www.w3.org/2004/02/skos/core#" rdf:about="http://inspire.ec.europa.eu/metadata-codelist/SpatialDataServiceCategory/humanGeographicSpreadsheetViewer">
    <skos:prefLabel xml:lang="en">Geographic spreadsheet viewer</skos:prefLabel>
    <skos:scopeNote xml:lang="en">Client service that allows a user to interact with multiple data objects and to request calculations similar to an arithmetic spreadsheet but extended to geographic data.</skos:scopeNote>
    <skos:prefLabel xml:lang="es">Visor geográfico de hoja de cálculo</skos:prefLabel>
    <skos:scopeNote xml:lang="es">Servicio cliente que permite al usuario interactuar con múltiples objetos de datos y solicitar cálculos similares a los de una hoja de cálculo aritmético pero extendidos a datos geográficos.</skos:scopeNote>
    <skos:prefLabel xml:lang="fr">Service de visualisation de feuilles de calcul géographiques</skos:prefLabel>
    <skos:scopeNote xml:lang="fr">Service client permettant l’interaction de l’utilisateur avec plusieurs objets de données; l’utilisateur peut également demander des calculs analogues à ceux d’une feuille de calcul arithmétique, mais étendus à des données géographiques.</skos:scopeNote>
    <skos:prefLabel xml:lang="pt">Visualização de folhas de cálculo geográficas</skos:prefLabel>
    <skos:scopeNote xml:lang="pt">Serviço cliente que permite ao utilizador interagir com múltiplos objectos de dados e solicitar cálculos semelhantes a uma folha de cálculo aritmética, mas alargada a dados geográficos.</skos:scopeNote>
    <skos:inScheme rdf:resource="http://inspire.ec.europa.eu/metadata-codelist/SpatialDataServiceCategory" />
    <skos:broader rdf:resource="http://inspire.ec.europa.eu/metadata-codelist/SpatialDataServiceCategory/humanInteractionService" />
  </skos:Concept>
  <skos:Concept xmlns:skos="http://www.w3.org/2004/02/skos/core#" rdf:about="http://inspire.ec.europa.eu/metadata-codelist/SpatialDataServiceCategory/humanServiceEditor">
    <skos:prefLabel xml:lang="en">Service editor</skos:prefLabel>
    <skos:scopeNote xml:lang="en">Client service that allows a user to control geographic processing services.</skos:scopeNote>
    <skos:prefLabel xml:lang="es">Editor de servicios</skos:prefLabel>
    <skos:scopeNote xml:lang="es">Servicio cliente que permite al usuario controlar servicios geográficos de procesamiento.</skos:scopeNote>
    <skos:prefLabel xml:lang="fr">Éditeur de services</skos:prefLabel>
    <skos:scopeNote xml:lang="fr">Service client permettant à l’utilisateur de contrôler les services de traitement géographique.</skos:scopeNote>
    <skos:prefLabel xml:lang="pt">Editor do serviço</skos:prefLabel>
    <skos:scopeNote xml:lang="pt">Serviço cliente que permite ao utilizador controlar serviços de processamento geográfico.</skos:scopeNote>
    <skos:inScheme rdf:resource="http://inspire.ec.europa.eu/metadata-codelist/SpatialDataServiceCategory" />
    <skos:broader rdf:resource="http://inspire.ec.europa.eu/metadata-codelist/SpatialDataServiceCategory/humanInteractionService" />
  </skos:Concept>
  <skos:Concept xmlns:skos="http://www.w3.org/2004/02/skos/core#" rdf:about="http://inspire.ec.europa.eu/metadata-codelist/SpatialDataServiceCategory/humanChainDefinitionEditor">
    <skos:prefLabel xml:lang="en">Chain definition editor</skos:prefLabel>
    <skos:scopeNote xml:lang="en">Provides user interaction with a chain definition service.</skos:scopeNote>
    <skos:prefLabel xml:lang="es">Editor de definición de cadenas</skos:prefLabel>
    <skos:scopeNote xml:lang="es">Este editor permite la interacción del usuario con un servicio de definición de cadenas.</skos:scopeNote>
    <skos:prefLabel xml:lang="fr">Éditeur pour la définition de chaînes</skos:prefLabel>
    <skos:scopeNote xml:lang="fr">Service permettant l’interaction de l’utilisateur avec un service de définition de chaînes.</skos:scopeNote>
    <skos:prefLabel xml:lang="pt">Editor da definição de cadeias</skos:prefLabel>
    <skos:scopeNote xml:lang="pt">Serviço que permite ao utilizador interagir com um serviço de definição de cadeias.</skos:scopeNote>
    <skos:inScheme rdf:resource="http://inspire.ec.europa.eu/metadata-codelist/SpatialDataServiceCategory" />
    <skos:broader rdf:resource="http://inspire.ec.europa.eu/metadata-codelist/SpatialDataServiceCategory/humanInteractionService" />
  </skos:Concept>
  <skos:Concept xmlns:skos="http://www.w3.org/2004/02/skos/core#" rdf:about="http://inspire.ec.europa.eu/metadata-codelist/SpatialDataServiceCategory/humanWorkflowEnactmentManager">
    <skos:prefLabel xml:lang="en">Workflow enactment manager</skos:prefLabel>
    <skos:scopeNote xml:lang="en">Provides user interaction with a workflow enactment service.</skos:scopeNote>
    <skos:prefLabel xml:lang="es">Gestor de lanzamiento de flujos de trabajo</skos:prefLabel>
    <skos:scopeNote xml:lang="es">Este gestor permite la interacción con un servicio de lanzamiento de flujos de trabajo.</skos:scopeNote>
    <skos:prefLabel xml:lang="fr">Gestionnaire de contrôle de processus</skos:prefLabel>
    <skos:scopeNote xml:lang="fr">Service permettant l’interaction de l’utilisateur avec un service de contrôle de processus.</skos:scopeNote>
    <skos:prefLabel xml:lang="pt">Gestor do fluxo de trabalho</skos:prefLabel>
    <skos:scopeNote xml:lang="pt">Serviço que permite ao utilizador interagir com um serviço de fluxo de trabalho.</skos:scopeNote>
    <skos:inScheme rdf:resource="http://inspire.ec.europa.eu/metadata-codelist/SpatialDataServiceCategory" />
    <skos:broader rdf:resource="http://inspire.ec.europa.eu/metadata-codelist/SpatialDataServiceCategory/humanInteractionService" />
  </skos:Concept>
  <skos:Concept xmlns:skos="http://www.w3.org/2004/02/skos/core#" rdf:about="http://inspire.ec.europa.eu/metadata-codelist/SpatialDataServiceCategory/humanGeographicFeatureEditor">
    <skos:prefLabel xml:lang="en">Geographic feature editor</skos:prefLabel>
    <skos:scopeNote xml:lang="en">Geographic viewer that allows a user to interact with feature data.</skos:scopeNote>
    <skos:prefLabel xml:lang="es">Editor de fenómenos geográficos</skos:prefLabel>
    <skos:scopeNote xml:lang="es">Visor geográfico que permite al usuario interactuar con datos de fenómenos.</skos:scopeNote>
    <skos:prefLabel xml:lang="fr">Éditeur d’éléments géographiques</skos:prefLabel>
    <skos:scopeNote xml:lang="fr">Visualiseur géographique permettant l’interaction de l’utilisateur avec les données relatives aux éléments géographiques.</skos:scopeNote>
    <skos:prefLabel xml:lang="pt">Editor de elementos geográficos</skos:prefLabel>
    <skos:scopeNote xml:lang="pt">Visualizador geográfico que permite ao utilizador interagir com os dados relativos aos elementos geográficos.</skos:scopeNote>
    <skos:inScheme rdf:resource="http://inspire.ec.europa.eu/metadata-codelist/SpatialDataServiceCategory" />
    <skos:broader rdf:resource="http://inspire.ec.europa.eu/metadata-codelist/SpatialDataServiceCategory/humanInteractionService" />
  </skos:Concept>
  <skos:Concept xmlns:skos="http://www.w3.org/2004/02/skos/core#" rdf:about="http://inspire.ec.europa.eu/metadata-codelist/SpatialDataServiceCategory/humanGeographicSymbolEditor">
    <skos:prefLabel xml:lang="en">Geographic symbol editor</skos:prefLabel>
    <skos:scopeNote xml:lang="en">Client service that allows a human to select and manage symbol libraries.</skos:scopeNote>
    <skos:prefLabel xml:lang="es">Editor de símbolos geográficos</skos:prefLabel>
    <skos:scopeNote xml:lang="es">Servicio cliente que permite a una persona seleccionar y gestionar bibliotecas de símbolos.</skos:scopeNote>
    <skos:prefLabel xml:lang="fr">Éditeur de symboles géographiques</skos:prefLabel>
    <skos:scopeNote xml:lang="fr">Service client permettant à un utilisateur humain de sélectionner et de gérer des bibliothèques de symboles.</skos:scopeNote>
    <skos:prefLabel xml:lang="pt">Editor de símbolos geográficos</skos:prefLabel>
    <skos:scopeNote xml:lang="pt">Serviço cliente que permite ao utilizador seleccionar e gerir bibliotecas de símbolos.</skos:scopeNote>
    <skos:inScheme rdf:resource="http://inspire.ec.europa.eu/metadata-codelist/SpatialDataServiceCategory" />
    <skos:broader rdf:resource="http://inspire.ec.europa.eu/metadata-codelist/SpatialDataServiceCategory/humanInteractionService" />
  </skos:Concept>
  <skos:Concept xmlns:skos="http://www.w3.org/2004/02/skos/core#" rdf:about="http://inspire.ec.europa.eu/metadata-codelist/SpatialDataServiceCategory/humanFeatureGeneralizationEditor">
    <skos:prefLabel xml:lang="en">Feature generalisation editor</skos:prefLabel>
    <skos:scopeNote xml:lang="en">Client service that allows a user to modify the cartographic characteristics of a feature or feature collection by simplifying its visualisation, while maintaining its salient elements – the spatial equivalent of simplification.</skos:scopeNote>
    <skos:prefLabel xml:lang="es">Editor de generalización de fenómenos</skos:prefLabel>
    <skos:scopeNote xml:lang="es">Servicio cliente que permite al usuario modificar las características cartográficas de un fenómeno o colección de fenómenos simplificando su visualización pero manteniendo sus elementos más destacados (equivalente espacial de la simplificación).</skos:scopeNote>
    <skos:prefLabel xml:lang="fr">Éditeur de généralisation d’éléments</skos:prefLabel>
    <skos:scopeNote xml:lang="fr">Service client permettant à l’utilisateur de modifier les caractéristiques cartographiques d’un élément ou d’une compilation d’éléments en simplifiant leur visualisation, tout en conservant les éléments essentiels, ce qui correspond à l’équivalent spatial de la simplification.</skos:scopeNote>
    <skos:prefLabel xml:lang="pt">Editor de generalização de elementos geográficos</skos:prefLabel>
    <skos:scopeNote xml:lang="pt">Serviço cliente que permite ao utilizador modificar as características cartográficas de um elemento geográfico ou colecção de elementos geográficos simplificando a sua visualização, mas mantendo simultaneamente as suas componentes relevantes — o equivalente espacial de simplificação.</skos:scopeNote>
    <skos:inScheme rdf:resource="http://inspire.ec.europa.eu/metadata-codelist/SpatialDataServiceCategory" />
    <skos:broader rdf:resource="http://inspire.ec.europa.eu/metadata-codelist/SpatialDataServiceCategory/humanInteractionService" />
  </skos:Concept>
  <skos:Concept xmlns:skos="http://www.w3.org/2004/02/skos/core#" rdf:about="http://inspire.ec.europa.eu/metadata-codelist/SpatialDataServiceCategory/humanGeographicDataStructureViewer">
    <skos:prefLabel xml:lang="en">Geographic data-structure viewer</skos:prefLabel>
    <skos:scopeNote xml:lang="en">Client service that allows a user to access part of data set to see its internal structure.</skos:scopeNote>
    <skos:prefLabel xml:lang="es">Visor de estructuras de datos geográficos</skos:prefLabel>
    <skos:scopeNote xml:lang="es">Servicio cliente que permite al usuario acceder a una parte de un conjunto de datos para ver su estructura interna.</skos:scopeNote>
    <skos:prefLabel xml:lang="fr">Visualiseur de la structure des données géographiques</skos:prefLabel>
    <skos:scopeNote xml:lang="fr">Service client permettant à l’utilisateur d’accéder à une partie de série de données pour en voir la structure interne.</skos:scopeNote>
    <skos:prefLabel xml:lang="pt">Visualizador da estrutura dos dados geográficos</skos:prefLabel>
    <skos:scopeNote xml:lang="pt">Serviço cliente que permite ao utilizador aceder a parte do conjunto de dados para ver a respectiva estrutura interna.</skos:scopeNote>
    <skos:inScheme rdf:resource="http://inspire.ec.europa.eu/metadata-codelist/SpatialDataServiceCategory" />
    <skos:broader rdf:resource="http://inspire.ec.europa.eu/metadata-codelist/SpatialDataServiceCategory/humanInteractionService" />
  </skos:Concept>
  <skos:Concept xmlns:skos="http://www.w3.org/2004/02/skos/core#" rdf:about="http://inspire.ec.europa.eu/metadata-codelist/SpatialDataServiceCategory/infoManagementService">
    <skos:prefLabel xml:lang="en">Geographic model/information management service</skos:prefLabel>
    <skos:prefLabel xml:lang="es">Servicio de gestión de modelos/información geográficos</skos:prefLabel>
    <skos:prefLabel xml:lang="fr">Services de gestion des modèles/informations géographiques</skos:prefLabel>
    <skos:prefLabel xml:lang="pt">Serviço de gestão de informação/modelos geográficos</skos:prefLabel>
    <skos:inScheme rdf:resource="http://inspire.ec.europa.eu/metadata-codelist/SpatialDataServiceCategory" />
    <skos:narrower rdf:resource="http://inspire.ec.europa.eu/metadata-codelist/SpatialDataServiceCategory/infoFeatureAccessService" />
    <skos:narrower rdf:resource="http://inspire.ec.europa.eu/metadata-codelist/SpatialDataServiceCategory/infoMapAccessService" />
    <skos:narrower rdf:resource="http://inspire.ec.europa.eu/metadata-codelist/SpatialDataServiceCategory/infoCoverageAccessService" />
    <skos:narrower rdf:resource="http://inspire.ec.europa.eu/metadata-codelist/SpatialDataServiceCategory/infoSensorDescriptionService" />
    <skos:narrower rdf:resource="http://inspire.ec.europa.eu/metadata-codelist/SpatialDataServiceCategory/infoProductAccessService" />
    <skos:narrower rdf:resource="http://inspire.ec.europa.eu/metadata-codelist/SpatialDataServiceCategory/infoFeatureTypeService" />
    <skos:narrower rdf:resource="http://inspire.ec.europa.eu/metadata-codelist/SpatialDataServiceCategory/infoCatalogueService" />
    <skos:narrower rdf:resource="http://inspire.ec.europa.eu/metadata-codelist/SpatialDataServiceCategory/infoRegistryService" />
    <skos:narrower rdf:resource="http://inspire.ec.europa.eu/metadata-codelist/SpatialDataServiceCategory/infoGazetteerService" />
    <skos:narrower rdf:resource="http://inspire.ec.europa.eu/metadata-codelist/SpatialDataServiceCategory/infoOrderHandlingService" />
    <skos:narrower rdf:resource="http://inspire.ec.europa.eu/metadata-codelist/SpatialDataServiceCategory/infoStandingOrderService" />
  </skos:Concept>
  <skos:Concept xmlns:skos="http://www.w3.org/2004/02/skos/core#" rdf:about="http://inspire.ec.europa.eu/metadata-codelist/SpatialDataServiceCategory/infoFeatureAccessService">
    <skos:prefLabel xml:lang="en">Feature access service</skos:prefLabel>
    <skos:scopeNote xml:lang="en">Service that provides a client access to and management of a feature store.</skos:scopeNote>
    <skos:prefLabel xml:lang="es">Servicio de acceso a fenómenos</skos:prefLabel>
    <skos:scopeNote xml:lang="es">Servicio que permite al cliente acceder a un almacén de fenómenos y gestionarlo.</skos:scopeNote>
    <skos:prefLabel xml:lang="fr">Service d’accès aux éléments</skos:prefLabel>
    <skos:scopeNote xml:lang="fr">Service permettant au client d’accéder à un magasin d’éléments et de le gérer.</skos:scopeNote>
    <skos:prefLabel xml:lang="pt">Serviço de acesso a elementos geográficos</skos:prefLabel>
    <skos:scopeNote xml:lang="pt">Serviço que permite ao cliente o acesso e a gestão de um repositório de elementos geográficos.</skos:scopeNote>
    <skos:inScheme rdf:resource="http://inspire.ec.europa.eu/metadata-codelist/SpatialDataServiceCategory" />
    <skos:broader rdf:resource="http://inspire.ec.europa.eu/metadata-codelist/SpatialDataServiceCategory/infoManagementService" />
  </skos:Concept>
  <skos:Concept xmlns:skos="http://www.w3.org/2004/02/skos/core#" rdf:about="http://inspire.ec.europa.eu/metadata-codelist/SpatialDataServiceCategory/infoMapAccessService">
    <skos:prefLabel xml:lang="en">Map access service</skos:prefLabel>
    <skos:scopeNote xml:lang="en">Service that provides a client access to a geographic graphics, i.e. pictures of geographic data.</skos:scopeNote>
    <skos:prefLabel xml:lang="es">Servicio de acceso a mapas</skos:prefLabel>
    <skos:scopeNote xml:lang="es">Servicio que permite a un cliente acceder a gráficos geográficos, es decir, a imágenes de datos geográficos.</skos:scopeNote>
    <skos:prefLabel xml:lang="fr">Service d’accès aux cartes</skos:prefLabel>
    <skos:scopeNote xml:lang="fr">Service permettant au client d’accéder à des graphiques géographiques, c’est-à-dire à des représentations de données géographiques.</skos:scopeNote>
    <skos:prefLabel xml:lang="pt">Serviço de acesso a mapas</skos:prefLabel>
    <skos:scopeNote xml:lang="pt">Serviço que permite ao cliente o acesso a representações gráficas dos dados geográficos, ou seja, imagens de dados geográficos.</skos:scopeNote>
    <skos:inScheme rdf:resource="http://inspire.ec.europa.eu/metadata-codelist/SpatialDataServiceCategory" />
    <skos:broader rdf:resource="http://inspire.ec.europa.eu/metadata-codelist/SpatialDataServiceCategory/infoManagementService" />
  </skos:Concept>
  <skos:Concept xmlns:skos="http://www.w3.org/2004/02/skos/core#" rdf:about="http://inspire.ec.europa.eu/metadata-codelist/SpatialDataServiceCategory/infoCoverageAccessService">
    <skos:prefLabel xml:lang="en">Coverage access service</skos:prefLabel>
    <skos:scopeNote xml:lang="en">Service that provides a client access to and management of a coverage store.</skos:scopeNote>
    <skos:prefLabel xml:lang="es">Servicio de acceso a coberturas</skos:prefLabel>
    <skos:scopeNote xml:lang="es">Servicio que permite al cliente acceder a un almacén de coberturas y gestionarlo.</skos:scopeNote>
    <skos:prefLabel xml:lang="fr">Service d’accès aux couvertures</skos:prefLabel>
    <skos:scopeNote xml:lang="fr">Service permettant au client d’accéder à un magasin de couvertures et de le gérer.</skos:scopeNote>
    <skos:prefLabel xml:lang="pt">Serviço de acesso a coberturas</skos:prefLabel>
    <skos:scopeNote xml:lang="pt">Serviço que permite ao cliente o acesso e gestão de um repositório de coberturas.</skos:scopeNote>
    <skos:inScheme rdf:resource="http://inspire.ec.europa.eu/metadata-codelist/SpatialDataServiceCategory" />
    <skos:broader rdf:resource="http://inspire.ec.europa.eu/metadata-codelist/SpatialDataServiceCategory/infoManagementService" />
  </skos:Concept>
  <skos:Concept xmlns:skos="http://www.w3.org/2004/02/skos/core#" rdf:about="http://inspire.ec.europa.eu/metadata-codelist/SpatialDataServiceCategory/infoSensorDescriptionService">
    <skos:prefLabel xml:lang="en">Sensor description service</skos:prefLabel>
    <skos:scopeNote xml:lang="en">Service that provides the description of a coverage sensor, including sensor location and orientation, as well as the sensor’s geometric, dynamic, and radiometric characteristics for geo-processing purposes.</skos:scopeNote>
    <skos:prefLabel xml:lang="es">Servicio de descripción de sensores</skos:prefLabel>
    <skos:scopeNote xml:lang="es">Servicio que suministra la descripción de un sensor de coberturas, incluyendo la localización y orientación del sensor, así como las características geométricas, dinámicas y radiométricas con fines de geoprocesamiento.</skos:scopeNote>
    <skos:prefLabel xml:lang="fr">Service de description des capteurs</skos:prefLabel>
    <skos:scopeNote xml:lang="fr">Service fournissant la description des capteurs de couvertures à des fins de géotraitement. La description comprend notamment la position et l’orientation des capteurs ainsi que leurs caractéristiques géométriques, dynamiques et radiométriques.</skos:scopeNote>
    <skos:prefLabel xml:lang="pt">Serviço de descrição de sensores</skos:prefLabel>
    <skos:scopeNote xml:lang="pt">Serviço que fornece a descrição de um sensor de cobertura, incluindo a localização e orientação do sensor, bem como as características geométricas, dinâmicas e radiométricas do sensor, para fins de geoprocessamento.</skos:scopeNote>
    <skos:inScheme rdf:resource="http://inspire.ec.europa.eu/metadata-codelist/SpatialDataServiceCategory" />
    <skos:broader rdf:resource="http://inspire.ec.europa.eu/metadata-codelist/SpatialDataServiceCategory/infoManagementService" />
  </skos:Concept>
  <skos:Concept xmlns:skos="http://www.w3.org/2004/02/skos/core#" rdf:about="http://inspire.ec.europa.eu/metadata-codelist/SpatialDataServiceCategory/infoProductAccessService">
    <skos:prefLabel xml:lang="en">Product access service</skos:prefLabel>
    <skos:scopeNote xml:lang="en">Service that provides access to and management of a geographic product store.</skos:scopeNote>
    <skos:prefLabel xml:lang="es">Servicio de acceso a productos</skos:prefLabel>
    <skos:scopeNote xml:lang="es">Servicio que permite acceder a un almacén de productos geográficos y gestionarlo.</skos:scopeNote>
    <skos:prefLabel xml:lang="fr">Service d’accès aux produits</skos:prefLabel>
    <skos:scopeNote xml:lang="fr">Service permettant d’accéder à un magasin de produits géographiques et de le gérer.</skos:scopeNote>
    <skos:prefLabel xml:lang="pt">Serviço de acesso a produtos</skos:prefLabel>
    <skos:scopeNote xml:lang="pt">Serviço que permite o acesso e gestão de um repositório de produtos geográficos.</skos:scopeNote>
    <skos:inScheme rdf:resource="http://inspire.ec.europa.eu/metadata-codelist/SpatialDataServiceCategory" />
    <skos:broader rdf:resource="http://inspire.ec.europa.eu/metadata-codelist/SpatialDataServiceCategory/infoManagementService" />
  </skos:Concept>
  <skos:Concept xmlns:skos="http://www.w3.org/2004/02/skos/core#" rdf:about="http://inspire.ec.europa.eu/metadata-codelist/SpatialDataServiceCategory/infoFeatureTypeService">
    <skos:prefLabel xml:lang="en">Feature type service</skos:prefLabel>
    <skos:scopeNote xml:lang="en">Service that provides a client to access to and management of a store of feature type definitions.</skos:scopeNote>
    <skos:prefLabel xml:lang="es">Servicio de tipos de fenómenos</skos:prefLabel>
    <skos:scopeNote xml:lang="es">Servicio que permite al cliente acceder a un almacén de definiciones de tipos de fenómenos y gestionarlo.</skos:scopeNote>
    <skos:prefLabel xml:lang="fr">Service de types d’éléments</skos:prefLabel>
    <skos:scopeNote xml:lang="fr">Service permettant au client d’accéder à un magasin de définitions de types d’éléments et de le gérer.</skos:scopeNote>
    <skos:prefLabel xml:lang="pt">Serviço de tipos de elementos geográficos</skos:prefLabel>
    <skos:scopeNote xml:lang="pt">Serviço que permite ao cliente o acesso e gestão de um repositório de definições de tipos de elementos geográficos.</skos:scopeNote>
    <skos:inScheme rdf:resource="http://inspire.ec.europa.eu/metadata-codelist/SpatialDataServiceCategory" />
    <skos:broader rdf:resource="http://inspire.ec.europa.eu/metadata-codelist/SpatialDataServiceCategory/infoManagementService" />
  </skos:Concept>
  <skos:Concept xmlns:skos="http://www.w3.org/2004/02/skos/core#" rdf:about="http://inspire.ec.europa.eu/metadata-codelist/SpatialDataServiceCategory/infoCatalogueService">
    <skos:prefLabel xml:lang="en">Catalogue service</skos:prefLabel>
    <skos:scopeNote xml:lang="en">Service that provides discovery and management services on a store of metadata about instances.</skos:scopeNote>
    <skos:prefLabel xml:lang="es">Servicio de catálogo</skos:prefLabel>
    <skos:scopeNote xml:lang="es">Servicio que suministra servicios de localización y gestión en un almacén de metadatos acerca de instancias.</skos:scopeNote>
    <skos:prefLabel xml:lang="fr">Service de catalogue</skos:prefLabel>
    <skos:scopeNote xml:lang="fr">Service permettant de rechercher des métadonnées dans un magasin de métadonnées sur les ressources d’information, et de le gérer.</skos:scopeNote>
    <skos:prefLabel xml:lang="pt">Serviço de catálogo</skos:prefLabel>
    <skos:scopeNote xml:lang="pt">Serviço que oferece serviços de pesquisa e gestão num repositório de metadados sobre ocorrências.</skos:scopeNote>
    <skos:inScheme rdf:resource="http://inspire.ec.europa.eu/metadata-codelist/SpatialDataServiceCategory" />
    <skos:broader rdf:resource="http://inspire.ec.europa.eu/metadata-codelist/SpatialDataServiceCategory/infoManagementService" />
  </skos:Concept>
  <skos:Concept xmlns:skos="http://www.w3.org/2004/02/skos/core#" rdf:about="http://inspire.ec.europa.eu/metadata-codelist/SpatialDataServiceCategory/infoRegistryService">
    <skos:prefLabel xml:lang="en">Registry Service</skos:prefLabel>
    <skos:scopeNote xml:lang="en">Service that provides access to store of metadata about types.</skos:scopeNote>
    <skos:prefLabel xml:lang="es">Servicio de registro</skos:prefLabel>
    <skos:scopeNote xml:lang="es">Servicio que suministra acceso a un almacén de metadatos sobre tipos.</skos:scopeNote>
    <skos:prefLabel xml:lang="fr">Service de registre</skos:prefLabel>
    <skos:scopeNote xml:lang="fr">Service permettant d’accéder à un magasin de métadonnées sur les catégories de ressources d’information.</skos:scopeNote>
    <skos:prefLabel xml:lang="pt">Serviço de registo</skos:prefLabel>
    <skos:scopeNote xml:lang="pt">Serviço que permite o acesso a repositórios de metadados sobre tipos.</skos:scopeNote>
    <skos:inScheme rdf:resource="http://inspire.ec.europa.eu/metadata-codelist/SpatialDataServiceCategory" />
    <skos:broader rdf:resource="http://inspire.ec.europa.eu/metadata-codelist/SpatialDataServiceCategory/infoManagementService" />
  </skos:Concept>
  <skos:Concept xmlns:skos="http://www.w3.org/2004/02/skos/core#" rdf:about="http://inspire.ec.europa.eu/metadata-codelist/SpatialDataServiceCategory/infoGazetteerService">
    <skos:prefLabel xml:lang="en">Gazetteer service</skos:prefLabel>
    <skos:scopeNote xml:lang="en">Service that provides access to a directory of instances of a class or classes of real-world phenomena containing some information regarding position.</skos:scopeNote>
    <skos:prefLabel xml:lang="es">Servicio de nomenclátor</skos:prefLabel>
    <skos:scopeNote xml:lang="es">Servicio que da acceso a un directorio de instancias de una o varias clases de fenómenos del mundo real que contienen alguna información sobre su posición.</skos:scopeNote>
    <skos:prefLabel xml:lang="fr">Service toponymique</skos:prefLabel>
    <skos:scopeNote xml:lang="fr">Service permettant d’accéder à un répertoire d’occurrences d’une ou plusieurs catégories de phénomènes du monde réel contenant des informations ayant trait à la position.</skos:scopeNote>
    <skos:prefLabel xml:lang="pt">Serviço de repertório</skos:prefLabel>
    <skos:scopeNote xml:lang="pt">Serviço que permite o acesso a um directório de ocorrências de uma ou várias classes de fenómenos do mundo real com alguma informação relativa à posição.</skos:scopeNote>
    <skos:inScheme rdf:resource="http://inspire.ec.europa.eu/metadata-codelist/SpatialDataServiceCategory" />
    <skos:broader rdf:resource="http://inspire.ec.europa.eu/metadata-codelist/SpatialDataServiceCategory/infoManagementService" />
  </skos:Concept>
  <skos:Concept xmlns:skos="http://www.w3.org/2004/02/skos/core#" rdf:about="http://inspire.ec.europa.eu/metadata-codelist/SpatialDataServiceCategory/infoOrderHandlingService">
    <skos:prefLabel xml:lang="en">Order handling service</skos:prefLabel>
    <skos:scopeNote xml:lang="en">Service that provides a client with the ability to order products from a provider.</skos:scopeNote>
    <skos:prefLabel xml:lang="es">Servicio de gestión de pedidos</skos:prefLabel>
    <skos:scopeNote xml:lang="es">Servicio que permite al cliente pedir productos a un proveedor.</skos:scopeNote>
    <skos:prefLabel xml:lang="fr">Service de gestion des commandes</skos:prefLabel>
    <skos:scopeNote xml:lang="fr">Service permettant aux clients de commander des produits auprès d’un fournisseur.</skos:scopeNote>
    <skos:prefLabel xml:lang="pt">Serviço de gestão de encomendas</skos:prefLabel>
    <skos:scopeNote xml:lang="pt">Serviço que permite ao cliente encomendar produtos de um fornecedor.</skos:scopeNote>
    <skos:inScheme rdf:resource="http://inspire.ec.europa.eu/metadata-codelist/SpatialDataServiceCategory" />
    <skos:broader rdf:resource="http://inspire.ec.europa.eu/metadata-codelist/SpatialDataServiceCategory/infoManagementService" />
  </skos:Concept>
  <skos:Concept xmlns:skos="http://www.w3.org/2004/02/skos/core#" rdf:about="http://inspire.ec.europa.eu/metadata-codelist/SpatialDataServiceCategory/infoStandingOrderService">
    <skos:prefLabel xml:lang="en">Standing order service</skos:prefLabel>
    <skos:scopeNote xml:lang="en">Order handling service that allows a user to request that a product over a geographic area be disseminated when it becomes available.</skos:scopeNote>
    <skos:prefLabel xml:lang="es">Servicio de pedidos permanente</skos:prefLabel>
    <skos:scopeNote xml:lang="es">Servicio de gestión de pedidos que permite al usuario solicitar que se reparta un producto en una zona geográfica cuando esté disponible.</skos:scopeNote>
    <skos:prefLabel xml:lang="fr">Service de commande en attente</skos:prefLabel>
    <skos:scopeNote xml:lang="fr">Service de gestion des commandes permettant à l’utilisateur de demander qu’un produit couvrant une zone géographique déterminée soit diffusé lorsqu’il devient disponible.</skos:scopeNote>
    <skos:prefLabel xml:lang="pt">Serviço de encomendas pendentes</skos:prefLabel>
    <skos:scopeNote xml:lang="pt">Serviço de gestão de encomendas que permite ao utilizador solicitar que um produto sobre uma zona geográfica seja difundido logo que ficar disponível.</skos:scopeNote>
    <skos:inScheme rdf:resource="http://inspire.ec.europa.eu/metadata-codelist/SpatialDataServiceCategory" />
    <skos:broader rdf:resource="http://inspire.ec.europa.eu/metadata-codelist/SpatialDataServiceCategory/infoManagementService" />
  </skos:Concept>
  <skos:Concept xmlns:skos="http://www.w3.org/2004/02/skos/core#" rdf:about="http://inspire.ec.europa.eu/metadata-codelist/SpatialDataServiceCategory/taskManagementService">
    <skos:prefLabel xml:lang="en">Geographic workflow/task management services</skos:prefLabel>
    <skos:prefLabel xml:lang="es">Servicios de gestión de flujos de trabajo/tareas en el ámbito geográfico</skos:prefLabel>
    <skos:prefLabel xml:lang="fr">Services de gestion du processus/des tâches géographiques</skos:prefLabel>
    <skos:prefLabel xml:lang="pt">Serviços de gestão do fluxo de trabalho/tarefas geográficas</skos:prefLabel>
    <skos:inScheme rdf:resource="http://inspire.ec.europa.eu/metadata-codelist/SpatialDataServiceCategory" />
    <skos:narrower rdf:resource="http://inspire.ec.europa.eu/metadata-codelist/SpatialDataServiceCategory/chainDefinitionService" />
    <skos:narrower rdf:resource="http://inspire.ec.europa.eu/metadata-codelist/SpatialDataServiceCategory/workflowEnactmentService" />
    <skos:narrower rdf:resource="http://inspire.ec.europa.eu/metadata-codelist/SpatialDataServiceCategory/subscriptionService" />
  </skos:Concept>
  <skos:Concept xmlns:skos="http://www.w3.org/2004/02/skos/core#" rdf:about="http://inspire.ec.europa.eu/metadata-codelist/SpatialDataServiceCategory/chainDefinitionService">
    <skos:prefLabel xml:lang="en">Chain definition service</skos:prefLabel>
    <skos:scopeNote xml:lang="en">Service to define a chain and to enable it to be executed by the workflow enactment service.</skos:scopeNote>
    <skos:prefLabel xml:lang="es">Servicio de definición de cadenas</skos:prefLabel>
    <skos:scopeNote xml:lang="es">Servicio que define una cadena y permite ejecutarla mediante el servicio de lanzamiento de un flujo de trabajo.</skos:scopeNote>
    <skos:prefLabel xml:lang="fr">Service de définition de chaîne</skos:prefLabel>
    <skos:scopeNote xml:lang="fr">Service permettant de définir une chaîne et de la faire exécuter par le service de contrôle de processus.</skos:scopeNote>
    <skos:prefLabel xml:lang="pt">Serviço de definição de cadeia</skos:prefLabel>
    <skos:scopeNote xml:lang="pt">Serviço que permite definir uma cadeia e fazê-la executar pelo serviço de fluxo de trabalho.</skos:scopeNote>
    <skos:inScheme rdf:resource="http://inspire.ec.europa.eu/metadata-codelist/SpatialDataServiceCategory" />
    <skos:broader rdf:resource="http://inspire.ec.europa.eu/metadata-codelist/SpatialDataServiceCategory/taskManagementService" />
  </skos:Concept>
  <skos:Concept xmlns:skos="http://www.w3.org/2004/02/skos/core#" rdf:about="http://inspire.ec.europa.eu/metadata-codelist/SpatialDataServiceCategory/workflowEnactmentService">
    <skos:prefLabel xml:lang="en">Workflow enactment service</skos:prefLabel>
    <skos:scopeNote xml:lang="en">The workflow enactment service interprets a chain and controls the instantiation of services and sequencing of activities.</skos:scopeNote>
    <skos:prefLabel xml:lang="es">Servicio de lanzamiento de un flujo de trabajo</skos:prefLabel>
    <skos:scopeNote xml:lang="es">El servicio de lanzamiento de un flujo de trabajo interpreta una cadena y controla la instanciación de los servicios y la secuencia de las actividades.</skos:scopeNote>
    <skos:prefLabel xml:lang="fr">Service de contrôle de processus</skos:prefLabel>
    <skos:scopeNote xml:lang="fr">Le service de contrôle de processus interprète une chaîne et contrôle l’exécution des services et le séquençage des activités.</skos:scopeNote>
    <skos:prefLabel xml:lang="pt">Serviço de fluxo de trabalho</skos:prefLabel>
    <skos:scopeNote xml:lang="pt">O serviço de fluxo de trabalho interpreta uma cadeia e controla a instanciação de serviços e a sequenciação de actividades.</skos:scopeNote>
    <skos:inScheme rdf:resource="http://inspire.ec.europa.eu/metadata-codelist/SpatialDataServiceCategory" />
    <skos:broader rdf:resource="http://inspire.ec.europa.eu/metadata-codelist/SpatialDataServiceCategory/taskManagementService" />
  </skos:Concept>
  <skos:Concept xmlns:skos="http://www.w3.org/2004/02/skos/core#" rdf:about="http://inspire.ec.europa.eu/metadata-codelist/SpatialDataServiceCategory/subscriptionService">
    <skos:prefLabel xml:lang="en">Subscription service</skos:prefLabel>
    <skos:scopeNote xml:lang="en">Service to allow clients to register for notification about events.</skos:scopeNote>
    <skos:prefLabel xml:lang="es">Servicio de suscripción</skos:prefLabel>
    <skos:scopeNote xml:lang="es">Servicio que permite a los clientes registrarse para la notificación de eventos.</skos:scopeNote>
    <skos:prefLabel xml:lang="fr">Service d’abonnement</skos:prefLabel>
    <skos:scopeNote xml:lang="fr">Service permettant aux clients de s’abonner afin d’être informés des événements.</skos:scopeNote>
    <skos:prefLabel xml:lang="pt">Serviço de assinatura</skos:prefLabel>
    <skos:scopeNote xml:lang="pt">Serviço que permite aos clientes inscreverem-se para serem informados de eventos.</skos:scopeNote>
    <skos:inScheme rdf:resource="http://inspire.ec.europa.eu/metadata-codelist/SpatialDataServiceCategory" />
    <skos:broader rdf:resource="http://inspire.ec.europa.eu/metadata-codelist/SpatialDataServiceCategory/taskManagementService" />
  </skos:Concept>
  <skos:Concept xmlns:skos="http://www.w3.org/2004/02/skos/core#" rdf:about="http://inspire.ec.europa.eu/metadata-codelist/SpatialDataServiceCategory/spatialProcessingService">
    <skos:prefLabel xml:lang="en">Geographic processing services – spatial</skos:prefLabel>
    <skos:prefLabel xml:lang="es">Servicios geográficos de procesamiento de tipo espacial</skos:prefLabel>
    <skos:prefLabel xml:lang="fr">Services de traitement géographique — aspects spatiaux</skos:prefLabel>
    <skos:prefLabel xml:lang="pt">Serviços de processamento geográfico — elementos espaciais</skos:prefLabel>
    <skos:inScheme rdf:resource="http://inspire.ec.europa.eu/metadata-codelist/SpatialDataServiceCategory" />
    <skos:narrower rdf:resource="http://inspire.ec.europa.eu/metadata-codelist/SpatialDataServiceCategory/spatialCoordinateConversionService" />
    <skos:narrower rdf:resource="http://inspire.ec.europa.eu/metadata-codelist/SpatialDataServiceCategory/spatialCoordinateTransformationService" />
    <skos:narrower rdf:resource="http://inspire.ec.europa.eu/metadata-codelist/SpatialDataServiceCategory/spatialCoverageVectorConversionService" />
    <skos:narrower rdf:resource="http://inspire.ec.europa.eu/metadata-codelist/SpatialDataServiceCategory/spatialImageCoordinateConversionService" />
    <skos:narrower rdf:resource="http://inspire.ec.europa.eu/metadata-codelist/SpatialDataServiceCategory/spatialRectificationService" />
    <skos:narrower rdf:resource="http://inspire.ec.europa.eu/metadata-codelist/SpatialDataServiceCategory/spatialOrthorectificationService" />
    <skos:narrower rdf:resource="http://inspire.ec.europa.eu/metadata-codelist/SpatialDataServiceCategory/spatialSensorGeometryModelAdjustmentService" />
    <skos:narrower rdf:resource="http://inspire.ec.europa.eu/metadata-codelist/SpatialDataServiceCategory/spatialImageGeometryModelConversionService" />
    <skos:narrower rdf:resource="http://inspire.ec.europa.eu/metadata-codelist/SpatialDataServiceCategory/spatialSubsettingService" />
    <skos:narrower rdf:resource="http://inspire.ec.europa.eu/metadata-codelist/SpatialDataServiceCategory/spatialSamplingService" />
    <skos:narrower rdf:resource="http://inspire.ec.europa.eu/metadata-codelist/SpatialDataServiceCategory/spatialTilingChangeService" />
    <skos:narrower rdf:resource="http://inspire.ec.europa.eu/metadata-codelist/SpatialDataServiceCategory/spatialDimensionMeasurementService" />
    <skos:narrower rdf:resource="http://inspire.ec.europa.eu/metadata-codelist/SpatialDataServiceCategory/spatialFeatureManipulationService" />
    <skos:narrower rdf:resource="http://inspire.ec.europa.eu/metadata-codelist/SpatialDataServiceCategory/spatialFeatureMatchingService" />
    <skos:narrower rdf:resource="http://inspire.ec.europa.eu/metadata-codelist/SpatialDataServiceCategory/spatialFeatureGeneralizationService" />
    <skos:narrower rdf:resource="http://inspire.ec.europa.eu/metadata-codelist/SpatialDataServiceCategory/spatialRouteDeterminationService" />
    <skos:narrower rdf:resource="http://inspire.ec.europa.eu/metadata-codelist/SpatialDataServiceCategory/spatialPositioningService" />
    <skos:narrower rdf:resource="http://inspire.ec.europa.eu/metadata-codelist/SpatialDataServiceCategory/spatialProximityAnalysisService" />
  </skos:Concept>
  <skos:Concept xmlns:skos="http://www.w3.org/2004/02/skos/core#" rdf:about="http://inspire.ec.europa.eu/metadata-codelist/SpatialDataServiceCategory/spatialCoordinateConversionService">
    <skos:prefLabel xml:lang="en">Coordinate conversion service</skos:prefLabel>
    <skos:scopeNote xml:lang="en">Service to change coordinates from one coordinate system to another coordinate system that is related to the same datum.</skos:scopeNote>
    <skos:prefLabel xml:lang="es">Servicio de conversión de coordenadas</skos:prefLabel>
    <skos:scopeNote xml:lang="es">Servicio que cambia coordenadas de un sistema de coordenadas a otro relacionado con el mismo dato.</skos:scopeNote>
    <skos:prefLabel xml:lang="fr">Service de conversion des coordonnées</skos:prefLabel>
    <skos:scopeNote xml:lang="fr">Service permettant de modifier les coordonnées d’un système de coordonnées en coordonnées d’un autre système fondé sur le même datum géodésique.</skos:scopeNote>
    <skos:prefLabel xml:lang="pt">Serviço de conversão de coordenadas</skos:prefLabel>
    <skos:scopeNote xml:lang="pt">Serviço que permite modificar as coordenadas de um sistema de coordenadas para um outro sistema de coordenadas relacionado com o mesmo datum.</skos:scopeNote>
    <skos:inScheme rdf:resource="http://inspire.ec.europa.eu/metadata-codelist/SpatialDataServiceCategory" />
    <skos:broader rdf:resource="http://inspire.ec.europa.eu/metadata-codelist/SpatialDataServiceCategory/spatialProcessingService" />
  </skos:Concept>
  <skos:Concept xmlns:skos="http://www.w3.org/2004/02/skos/core#" rdf:about="http://inspire.ec.europa.eu/metadata-codelist/SpatialDataServiceCategory/spatialCoordinateTransformationService">
    <skos:prefLabel xml:lang="en">Coordinate transformation service</skos:prefLabel>
    <skos:scopeNote xml:lang="en">Service to change coordinates from a coordinate reference system based on one datum to a coordinate reference system based on a second datum.</skos:scopeNote>
    <skos:prefLabel xml:lang="es">Servicio de transformación de coordenadas</skos:prefLabel>
    <skos:scopeNote xml:lang="es">Servicio que cambia coordenadas de un sistema de referencia de coordenadas basado en un dato a otro sistema basado en otro dato diferente.</skos:scopeNote>
    <skos:prefLabel xml:lang="fr">Service de transformation des coordonnées</skos:prefLabel>
    <skos:scopeNote xml:lang="fr">Service permettant de modifier les coordonnées d’un système de référence fondé sur un datum géodésique en coordonnées d’un système de référence fondé sur un autre datum.</skos:scopeNote>
    <skos:prefLabel xml:lang="pt">Serviço de transformação de coordenadas</skos:prefLabel>
    <skos:scopeNote xml:lang="pt">Serviço que permite modificar as coordenadas de um sistema de referência de coordenadas baseado num datum para um sistema de referência de coordenadas baseado num segundo datum.</skos:scopeNote>
    <skos:inScheme rdf:resource="http://inspire.ec.europa.eu/metadata-codelist/SpatialDataServiceCategory" />
    <skos:broader rdf:resource="http://inspire.ec.europa.eu/metadata-codelist/SpatialDataServiceCategory/spatialProcessingService" />
  </skos:Concept>
  <skos:Concept xmlns:skos="http://www.w3.org/2004/02/skos/core#" rdf:about="http://inspire.ec.europa.eu/metadata-codelist/SpatialDataServiceCategory/spatialCoverageVectorConversionService">
    <skos:prefLabel xml:lang="en">Coverage/vector conversion service</skos:prefLabel>
    <skos:scopeNote xml:lang="en">Service to change the spatial representation from a coverage schema to a vector schema, or vice versa.</skos:scopeNote>
    <skos:prefLabel xml:lang="es">Servicio de conversión de cobertura/vector</skos:prefLabel>
    <skos:scopeNote xml:lang="es">Servicio que cambia la representación espacial de un esquema de cobertura a un esquema vectorial o viceversa.</skos:scopeNote>
    <skos:prefLabel xml:lang="fr">Service de conversion couverture/vecteur</skos:prefLabel>
    <skos:scopeNote xml:lang="fr">Service permettant de modifier la représentation spatiale pour passer d’un schéma de couverture à un schéma vectoriel, ou vice versa.</skos:scopeNote>
    <skos:prefLabel xml:lang="pt">Serviço de conversão cobertura/vector</skos:prefLabel>
    <skos:scopeNote xml:lang="pt">Serviço que permite mudar a representação espacial de um sistema de cobertura para um sistema vectorial, ou vice-versa.</skos:scopeNote>
    <skos:inScheme rdf:resource="http://inspire.ec.europa.eu/metadata-codelist/SpatialDataServiceCategory" />
    <skos:broader rdf:resource="http://inspire.ec.europa.eu/metadata-codelist/SpatialDataServiceCategory/spatialProcessingService" />
  </skos:Concept>
  <skos:Concept xmlns:skos="http://www.w3.org/2004/02/skos/core#" rdf:about="http://inspire.ec.europa.eu/metadata-codelist/SpatialDataServiceCategory/spatialImageCoordinateConversionService">
    <skos:prefLabel xml:lang="en">Image coordinate conversion service</skos:prefLabel>
    <skos:scopeNote xml:lang="en">A coordinate transformation or coordinate conversion service to change the coordinate reference system for an image.</skos:scopeNote>
    <skos:prefLabel xml:lang="es">Servicio de conversión de coordenadas de imagen</skos:prefLabel>
    <skos:scopeNote xml:lang="es">Servicio de conversión de coordenadas o de transformación de coordenadas que cambia el sistema de referencia de coordenadas de una imagen.</skos:scopeNote>
    <skos:prefLabel xml:lang="fr">Service de conversion des coordonnées des images</skos:prefLabel>
    <skos:scopeNote xml:lang="fr">Service de transformation ou de conversion des coordonnées permettant de modifier le système de référence des coordonnées pour une image.</skos:scopeNote>
    <skos:prefLabel xml:lang="pt">Serviço de conversão de coordenadas de imagens</skos:prefLabel>
    <skos:scopeNote xml:lang="pt">Um serviço de transformação de coordenadas ou de conversão de coordenadas que permite modificar o sistema de referência de coordenadas de uma imagem.</skos:scopeNote>
    <skos:inScheme rdf:resource="http://inspire.ec.europa.eu/metadata-codelist/SpatialDataServiceCategory" />
    <skos:broader rdf:resource="http://inspire.ec.europa.eu/metadata-codelist/SpatialDataServiceCategory/spatialProcessingService" />
  </skos:Concept>
  <skos:Concept xmlns:skos="http://www.w3.org/2004/02/skos/core#" rdf:about="http://inspire.ec.europa.eu/metadata-codelist/SpatialDataServiceCategory/spatialRectificationService">
    <skos:prefLabel xml:lang="en">Rectification service</skos:prefLabel>
    <skos:scopeNote xml:lang="en">Service for transforming an image into a perpendicular parallel projection and therefore a constant scale.</skos:scopeNote>
    <skos:prefLabel xml:lang="es">Servicio de rectificación</skos:prefLabel>
    <skos:scopeNote xml:lang="es">Servicio para la transformación de una imagen en una proyección paralela perpendicular y, por tanto, de escala constante.</skos:scopeNote>
    <skos:prefLabel xml:lang="fr">Service de rectification</skos:prefLabel>
    <skos:scopeNote xml:lang="fr">Service permettant de transformer une image en une projection parallèle perpendiculaire, et donc à une échelle constante.</skos:scopeNote>
    <skos:prefLabel xml:lang="pt">Serviço de rectificação</skos:prefLabel>
    <skos:scopeNote xml:lang="pt">Serviço que permite transformar uma imagem numa projecção paralela perpendicular e, por conseguinte, com uma escala constante.</skos:scopeNote>
    <skos:inScheme rdf:resource="http://inspire.ec.europa.eu/metadata-codelist/SpatialDataServiceCategory" />
    <skos:broader rdf:resource="http://inspire.ec.europa.eu/metadata-codelist/SpatialDataServiceCategory/spatialProcessingService" />
  </skos:Concept>
  <skos:Concept xmlns:skos="http://www.w3.org/2004/02/skos/core#" rdf:about="http://inspire.ec.europa.eu/metadata-codelist/SpatialDataServiceCategory/spatialOrthorectificationService">
    <skos:prefLabel xml:lang="en">Orthorectification service</skos:prefLabel>
    <skos:scopeNote xml:lang="en">A rectification service that removes image tilt and displacement due to terrain elevation.</skos:scopeNote>
    <skos:prefLabel xml:lang="es">Servicio de ortorrectificación</skos:prefLabel>
    <skos:scopeNote xml:lang="es">Servicio de rectificación que elimina las inclinaciones y los desplazamientos de la imagen debidos a la elevación del terreno.</skos:scopeNote>
    <skos:prefLabel xml:lang="fr">Service d’orthorectification</skos:prefLabel>
    <skos:scopeNote xml:lang="fr">Service de rectification qui élimine l’inclinaison et le décalage de l’image dû au relief du terrain.</skos:scopeNote>
    <skos:prefLabel xml:lang="pt">Serviço de ortorrectificação</skos:prefLabel>
    <skos:scopeNote xml:lang="pt">Um serviço de rectificação que corrige as deformações devidas ao ângulo de obtenção da imagem e os desvios da imagem decorrentes do relevo.</skos:scopeNote>
    <skos:inScheme rdf:resource="http://inspire.ec.europa.eu/metadata-codelist/SpatialDataServiceCategory" />
    <skos:broader rdf:resource="http://inspire.ec.europa.eu/metadata-codelist/SpatialDataServiceCategory/spatialProcessingService" />
  </skos:Concept>
  <skos:Concept xmlns:skos="http://www.w3.org/2004/02/skos/core#" rdf:about="http://inspire.ec.europa.eu/metadata-codelist/SpatialDataServiceCategory/spatialSensorGeometryModelAdjustmentService">
    <skos:prefLabel xml:lang="en">Sensor geometry model adjustment service</skos:prefLabel>
    <skos:scopeNote xml:lang="en">Service that adjusts sensor geometry models to improve the match of the image with other images and/or known ground positions.</skos:scopeNote>
    <skos:prefLabel xml:lang="es">Servicio de ajuste del modelo de geometría del sensor</skos:prefLabel>
    <skos:scopeNote xml:lang="es">Servicio que ajusta los modelos de geometría del sensor para mejorar el ajuste de la imagen con otras imágenes o posiciones conocidas en el terreno.</skos:scopeNote>
    <skos:prefLabel xml:lang="fr">Service d’ajustement des modèles géométriques des capteurs</skos:prefLabel>
    <skos:scopeNote xml:lang="fr">Service permettant d’ajuster les modèles géométriques des capteurs pour améliorer la concordance de l’image avec d’autres images et/ou positions au sol connues.</skos:scopeNote>
    <skos:prefLabel xml:lang="pt">Serviço de ajustamento do modelo geométrico dos sensores</skos:prefLabel>
    <skos:scopeNote xml:lang="pt">Serviço que permite ajustar os modelos geométricos dos sensores a fim de melhorar a correspondência da imagem com outras imagens e/ou posições no solo conhecidas.</skos:scopeNote>
    <skos:inScheme rdf:resource="http://inspire.ec.europa.eu/metadata-codelist/SpatialDataServiceCategory" />
    <skos:broader rdf:resource="http://inspire.ec.europa.eu/metadata-codelist/SpatialDataServiceCategory/spatialProcessingService" />
  </skos:Concept>
  <skos:Concept xmlns:skos="http://www.w3.org/2004/02/skos/core#" rdf:about="http://inspire.ec.europa.eu/metadata-codelist/SpatialDataServiceCategory/spatialImageGeometryModelConversionService">
    <skos:prefLabel xml:lang="en">Image geometry model conversion service</skos:prefLabel>
    <skos:scopeNote xml:lang="en">Service that converts sensor geometry models into a different but equivalent sensor geometry model.</skos:scopeNote>
    <skos:prefLabel xml:lang="es">Servicio de conversión del modelo de geometría de la imagen</skos:prefLabel>
    <skos:scopeNote xml:lang="es">Servicio que convierte el modelo de geometría del sensor en un modelo de geometría del sensor diferente pero equivalente.</skos:scopeNote>
    <skos:prefLabel xml:lang="fr">Service de conversion des modèles géométriques des images</skos:prefLabel>
    <skos:scopeNote xml:lang="fr">Service permettant de convertir les modèles géométriques des capteurs en un modèle géométrique différent, mais équivalent.</skos:scopeNote>
    <skos:prefLabel xml:lang="pt">Serviço de conversão de modelos geométricos das imagens</skos:prefLabel>
    <skos:scopeNote xml:lang="pt">Serviço que permite converter modelos geométricos dos sensores num modelo geométrico de sensores diferente, mas equivalente.</skos:scopeNote>
    <skos:inScheme rdf:resource="http://inspire.ec.europa.eu/metadata-codelist/SpatialDataServiceCategory" />
    <skos:broader rdf:resource="http://inspire.ec.europa.eu/metadata-codelist/SpatialDataServiceCategory/spatialProcessingService" />
  </skos:Concept>
  <skos:Concept xmlns:skos="http://www.w3.org/2004/02/skos/core#" rdf:about="http://inspire.ec.europa.eu/metadata-codelist/SpatialDataServiceCategory/spatialSubsettingService">
    <skos:prefLabel xml:lang="en">Subsetting service</skos:prefLabel>
    <skos:scopeNote xml:lang="en">Service that extracts data from an input in a continuous spatial region either by geographic location or by grid coordinates.</skos:scopeNote>
    <skos:prefLabel xml:lang="es">Servicio de subdivisión</skos:prefLabel>
    <skos:scopeNote xml:lang="es">Servicio que extrae datos de una entrada de una región espacial continua bien por localización geográfica bien por coordenadas de malla.</skos:scopeNote>
    <skos:prefLabel xml:lang="fr">Service de définition de sous-ensembles</skos:prefLabel>
    <skos:scopeNote xml:lang="fr">Service permettant d’extraire des données d’un ensemble spatial continu, sur la base soit de la position géographique, soit des coordonnées de la grille.</skos:scopeNote>
    <skos:prefLabel xml:lang="pt">Serviço de definição de subconjuntos</skos:prefLabel>
    <skos:scopeNote xml:lang="pt">Serviço que extrai dados de uma fonte numa região espacial contínua com base na localização geográfica ou em coordenadas rectangulares.</skos:scopeNote>
    <skos:inScheme rdf:resource="http://inspire.ec.europa.eu/metadata-codelist/SpatialDataServiceCategory" />
    <skos:broader rdf:resource="http://inspire.ec.europa.eu/metadata-codelist/SpatialDataServiceCategory/spatialProcessingService" />
  </skos:Concept>
  <skos:Concept xmlns:skos="http://www.w3.org/2004/02/skos/core#" rdf:about="http://inspire.ec.europa.eu/metadata-codelist/SpatialDataServiceCategory/spatialSamplingService">
    <skos:prefLabel xml:lang="en">Sampling service</skos:prefLabel>
    <skos:scopeNote xml:lang="en">Service that extracts data from an input using a consistent sampling scheme either by geographic location or by grid coordinates.</skos:scopeNote>
    <skos:prefLabel xml:lang="es">Servicio de muestreo</skos:prefLabel>
    <skos:scopeNote xml:lang="es">Servicio que extrae datos de una entrada usando un esquema de muestreo coherente bien por localización geográfica bien por coordenadas de malla.</skos:scopeNote>
    <skos:prefLabel xml:lang="fr">Service d’échantillonnage</skos:prefLabel>
    <skos:scopeNote xml:lang="fr">Service permettant d’extraire des données au moyen d’un système d’échantillonnage cohérent, sur la base soit de la position géographique, soit des coordonnées de la grille.</skos:scopeNote>
    <skos:prefLabel xml:lang="pt">Serviço de amostragem</skos:prefLabel>
    <skos:scopeNote xml:lang="pt">Serviço que extrai dados de uma fonte utilizando um sistema de amostragem coerente com base na localização geográfica ou em coordenadas rectangulares.</skos:scopeNote>
    <skos:inScheme rdf:resource="http://inspire.ec.europa.eu/metadata-codelist/SpatialDataServiceCategory" />
    <skos:broader rdf:resource="http://inspire.ec.europa.eu/metadata-codelist/SpatialDataServiceCategory/spatialProcessingService" />
  </skos:Concept>
  <skos:Concept xmlns:skos="http://www.w3.org/2004/02/skos/core#" rdf:about="http://inspire.ec.europa.eu/metadata-codelist/SpatialDataServiceCategory/spatialTilingChangeService">
    <skos:prefLabel xml:lang="en">Tiling change service</skos:prefLabel>
    <skos:scopeNote xml:lang="en">Service that changes the tiling of geographic data.</skos:scopeNote>
    <skos:prefLabel xml:lang="es">Servicio de cambio de división en hojas</skos:prefLabel>
    <skos:scopeNote xml:lang="es">Servicio que cambia la división en hojas de los datos geográficos.</skos:scopeNote>
    <skos:prefLabel xml:lang="fr">Service de modification du dallage</skos:prefLabel>
    <skos:scopeNote xml:lang="fr">Service permettant de modifier le dallage des données géographiques.</skos:scopeNote>
    <skos:prefLabel xml:lang="pt">Serviço de modificação do seccionamento</skos:prefLabel>
    <skos:scopeNote xml:lang="pt">Serviço que permite modificar o seccionamento dos dados geográficos.</skos:scopeNote>
    <skos:inScheme rdf:resource="http://inspire.ec.europa.eu/metadata-codelist/SpatialDataServiceCategory" />
    <skos:broader rdf:resource="http://inspire.ec.europa.eu/metadata-codelist/SpatialDataServiceCategory/spatialProcessingService" />
  </skos:Concept>
  <skos:Concept xmlns:skos="http://www.w3.org/2004/02/skos/core#" rdf:about="http://inspire.ec.europa.eu/metadata-codelist/SpatialDataServiceCategory/spatialDimensionMeasurementService">
    <skos:prefLabel xml:lang="en">Dimension measurement service</skos:prefLabel>
    <skos:scopeNote xml:lang="en">Service to compute dimensions of objects visible in an image or other geodata.</skos:scopeNote>
    <skos:prefLabel xml:lang="es">Servicio de medición de dimensiones</skos:prefLabel>
    <skos:scopeNote xml:lang="es">Servicio que calcula las dimensiones de objetos visibles en una imagen u otros datos geográficos.</skos:scopeNote>
    <skos:prefLabel xml:lang="fr">Service de mesure des dimensions</skos:prefLabel>
    <skos:scopeNote xml:lang="fr">Service qui calcule les dimensions des objets visibles sur une image ou sur d’autres données géographiques.</skos:scopeNote>
    <skos:prefLabel xml:lang="pt">Serviço de medição das dimensões</skos:prefLabel>
    <skos:scopeNote xml:lang="pt">Serviço que calcula as dimensões de objectos visíveis numa imagem ou noutros dados geográficos.</skos:scopeNote>
    <skos:inScheme rdf:resource="http://inspire.ec.europa.eu/metadata-codelist/SpatialDataServiceCategory" />
    <skos:broader rdf:resource="http://inspire.ec.europa.eu/metadata-codelist/SpatialDataServiceCategory/spatialProcessingService" />
  </skos:Concept>
  <skos:Concept xmlns:skos="http://www.w3.org/2004/02/skos/core#" rdf:about="http://inspire.ec.europa.eu/metadata-codelist/SpatialDataServiceCategory/spatialFeatureManipulationService">
    <skos:prefLabel xml:lang="en">Feature manipulation services</skos:prefLabel>
    <skos:scopeNote xml:lang="en">Register one feature to another, an image, or another data set or coordinate set; correcting for relative translation shifts, rotational differences, scale differences, and perspective differences. Verify that all features in the Feature Collection are topologically consistent according to the topology rules of the Feature Collection, and identifies and/or corrects any inconsistencies that are discovered.</skos:scopeNote>
    <skos:prefLabel xml:lang="es">Servicio de manipulación de fenómenos</skos:prefLabel>
    <skos:scopeNote xml:lang="es">Servicio que permite registrar un fenómeno respecto a otro, una imagen u otro conjunto de datos o de coordenadas, y corregir desplazamientos relativos, diferencias de rotación, diferencias de escala y diferencias de perspectiva. También permite verificar que todos los fenómenos de una colección de fenómenos sean topológicamente coherentes según las reglas de topología de la colección de fenómenos, y detectar o corregir cualquier incoherencia.</skos:scopeNote>
    <skos:prefLabel xml:lang="fr">Services de manipulation des éléments géographiques</skos:prefLabel>
    <skos:scopeNote xml:lang="fr">Ces services permettent de caler un élément sur un autre, sur une image, ou sur une autre série de données ou de coordonnées, de corriger les décalages relatifs, les différences de rotation, les différences d’échelle et les différences de perspective, de vérifier que tous les éléments figurant dans la compilation d’éléments sont topologiquement cohérents au regard des règles de topologie de la compilation d’éléments, et de recenser et/ou corriger les éventuelles incohérences décelées.</skos:scopeNote>
    <skos:prefLabel xml:lang="pt">Serviços de manipulação de elementos geográficos</skos:prefLabel>
    <skos:scopeNote xml:lang="pt">Estes serviços permitem inserir um elemento geográfico noutro elemento geográfico, imagem ou outro conjunto de dados ou conjunto de coordenadas, com correcção dos desvios translacionais relativos, das diferenças rotacionais, das diferenças de escala e das diferenças de perspectiva. Permitem verificar que todos os elementos geográficos da colecção de elementos geográficos são topologicamente coerentes de acordo com as regras topológicas da colecção de elementos e identifica e/ou corrige eventuais inconsistências detectadas.</skos:scopeNote>
    <skos:inScheme rdf:resource="http://inspire.ec.europa.eu/metadata-codelist/SpatialDataServiceCategory" />
    <skos:broader rdf:resource="http://inspire.ec.europa.eu/metadata-codelist/SpatialDataServiceCategory/spatialProcessingService" />
  </skos:Concept>
  <skos:Concept xmlns:skos="http://www.w3.org/2004/02/skos/core#" rdf:about="http://inspire.ec.europa.eu/metadata-codelist/SpatialDataServiceCategory/spatialFeatureMatchingService">
    <skos:prefLabel xml:lang="en">Feature matching service</skos:prefLabel>
    <skos:scopeNote xml:lang="en">Service that determines which features and portions of features represent the same real world entity from multiple data sources, e.g., edge matching and limited conflation.</skos:scopeNote>
    <skos:prefLabel xml:lang="es">Servicio de emparejamiento de fenómenos</skos:prefLabel>
    <skos:scopeNote xml:lang="es">Servicio que determina qué fenómenos y porciones de fenómenos representan la misma entidad del mundo real a partir de fuentes de datos múltiples, por ejemplo: correspondencia de bordes y conflación limitada.</skos:scopeNote>
    <skos:prefLabel xml:lang="fr">Service d’appariement d’éléments</skos:prefLabel>
    <skos:scopeNote xml:lang="fr">Service qui détermine quels éléments et parties d’éléments provenant de diverses sources de données représentent la même entité du monde réel, par exemple, appariement des contours et conflation limitée.</skos:scopeNote>
    <skos:prefLabel xml:lang="pt">Serviço de correspondência de elementos geográficos</skos:prefLabel>
    <skos:scopeNote xml:lang="pt">Serviço que determina quais são os elementos geográficos ou partes de elementos geográficos provenientes de múltiplas fontes de dados que representam a mesma entidade do mundo real, como acontece na coincidência de limites ("edge matching") e na fusão parcial de elementos geográficos ("limited conflation").</skos:scopeNote>
    <skos:inScheme rdf:resource="http://inspire.ec.europa.eu/metadata-codelist/SpatialDataServiceCategory" />
    <skos:broader rdf:resource="http://inspire.ec.europa.eu/metadata-codelist/SpatialDataServiceCategory/spatialProcessingService" />
  </skos:Concept>
  <skos:Concept xmlns:skos="http://www.w3.org/2004/02/skos/core#" rdf:about="http://inspire.ec.europa.eu/metadata-codelist/SpatialDataServiceCategory/spatialFeatureGeneralizationService">
    <skos:prefLabel xml:lang="en">Feature generalisation service</skos:prefLabel>
    <skos:scopeNote xml:lang="en">Service that reduces spatial variation in a feature collection to increase the effectiveness of communication by counteracting the undesirable effects of data reduction.</skos:scopeNote>
    <skos:prefLabel xml:lang="es">Servicio de generalización de fenómenos</skos:prefLabel>
    <skos:scopeNote xml:lang="es">Servicio que reduce la variación espacial de una colección de fenómenos para aumentar la eficacia de la comunicación al contrarrestar los efectos indeseables de la reducción de datos.</skos:scopeNote>
    <skos:prefLabel xml:lang="fr">Service de généralisation d’éléments</skos:prefLabel>
    <skos:scopeNote xml:lang="fr">Service qui réduit la variation spatiale dans une compilation d’éléments afin de renforcer l’efficacité de la communication en remédiant aux effets indésirables de la réduction de données.</skos:scopeNote>
    <skos:prefLabel xml:lang="pt">Serviço de generalização de elementos geográficos</skos:prefLabel>
    <skos:scopeNote xml:lang="pt">Serviço que reduz a variação espacial numa colecção de elementos geográficos a fim de aumentar a eficácia da comunicação mediante a neutralização dos efeitos indesejáveis da redução de dados.</skos:scopeNote>
    <skos:inScheme rdf:resource="http://inspire.ec.europa.eu/metadata-codelist/SpatialDataServiceCategory" />
    <skos:broader rdf:resource="http://inspire.ec.europa.eu/metadata-codelist/SpatialDataServiceCategory/spatialProcessingService" />
  </skos:Concept>
  <skos:Concept xmlns:skos="http://www.w3.org/2004/02/skos/core#" rdf:about="http://inspire.ec.europa.eu/metadata-codelist/SpatialDataServiceCategory/spatialRouteDeterminationService">
    <skos:prefLabel xml:lang="en">Route determination service</skos:prefLabel>
    <skos:scopeNote xml:lang="en">Service to determine the optimal path between two specified points based on the input parameters and properties contained in the Feature Collection.</skos:scopeNote>
    <skos:prefLabel xml:lang="es">Servicio de determinación de rutas</skos:prefLabel>
    <skos:scopeNote xml:lang="es">Servicio que determina el camino mínimo entre dos puntos dados basándose en los parámetros y propiedades de entrada contenidas en la colección de fenómenos.</skos:scopeNote>
    <skos:prefLabel xml:lang="fr">Service de détermination d’itinéraire</skos:prefLabel>
    <skos:scopeNote xml:lang="fr">Service qui, sur la base des paramètres d’entrée et des propriétés contenus dans la compilation d’éléments, détermine le trajet optimal entre deux points donnés.</skos:scopeNote>
    <skos:prefLabel xml:lang="pt">Serviço de determinação do itinerário</skos:prefLabel>
    <skos:scopeNote xml:lang="pt">Serviço que determina o trajecto óptimo entre dois pontos especificados com base nos parâmetros de entrada e nas propriedades contidas na colecção de elementos geográficos.</skos:scopeNote>
    <skos:inScheme rdf:resource="http://inspire.ec.europa.eu/metadata-codelist/SpatialDataServiceCategory" />
    <skos:broader rdf:resource="http://inspire.ec.europa.eu/metadata-codelist/SpatialDataServiceCategory/spatialProcessingService" />
  </skos:Concept>
  <skos:Concept xmlns:skos="http://www.w3.org/2004/02/skos/core#" rdf:about="http://inspire.ec.europa.eu/metadata-codelist/SpatialDataServiceCategory/spatialPositioningService">
    <skos:prefLabel xml:lang="en">Positioning service</skos:prefLabel>
    <skos:scopeNote xml:lang="en">Service provided by a position-providing device to use, obtain and unambiguously interpret position information, and determines whether the results meet the requirements of the use.</skos:scopeNote>
    <skos:prefLabel xml:lang="es">Servicio de posicionamiento</skos:prefLabel>
    <skos:scopeNote xml:lang="es">Servicio proporcionado por un dispositivo que suministra posiciones para usar, obtener e interpretar sin ambigüedad información sobre la posición; además este servicio determina si el resultado satisface los requisitos de uso.</skos:scopeNote>
    <skos:prefLabel xml:lang="fr">Service de positionnement</skos:prefLabel>
    <skos:scopeNote xml:lang="fr">Service fourni par un appareil de géopositionnement, permettant d’utiliser, d’obtenir et d’interpréter sans équivoque les informations concernant la position, ainsi que de déterminer si les résultats répondent aux exigences de l’utilisation.</skos:scopeNote>
    <skos:prefLabel xml:lang="pt">Serviço de localização</skos:prefLabel>
    <skos:scopeNote xml:lang="pt">Serviço fornecido por um dispositivo de localização que permite utilizar, obter e interpretar sem ambiguidades as informações relativas à localização e que determina se os resultados satisfazem os requisitos de utilização.</skos:scopeNote>
    <skos:inScheme rdf:resource="http://inspire.ec.europa.eu/metadata-codelist/SpatialDataServiceCategory" />
    <skos:broader rdf:resource="http://inspire.ec.europa.eu/metadata-codelist/SpatialDataServiceCategory/spatialProcessingService" />
  </skos:Concept>
  <skos:Concept xmlns:skos="http://www.w3.org/2004/02/skos/core#" rdf:about="http://inspire.ec.europa.eu/metadata-codelist/SpatialDataServiceCategory/spatialProximityAnalysisService">
    <skos:prefLabel xml:lang="en">Proximity analysis service</skos:prefLabel>
    <skos:scopeNote xml:lang="en">Given a position or geographic feature, finds all objects with a given set of attributes that are located within a user-specified distance of the position or feature.</skos:scopeNote>
    <skos:prefLabel xml:lang="es">Servicio de análisis de proximidad</skos:prefLabel>
    <skos:scopeNote xml:lang="es">Dada una posición o un fenómeno geográfico, este servicio encuentra todos los objetos con un conjunto dado de atributos que están localizados dentro de una distancia, especificada por el usuario, desde la posición o el fenómeno dado.</skos:scopeNote>
    <skos:prefLabel xml:lang="fr">Service d’analyse de proximité</skos:prefLabel>
    <skos:scopeNote xml:lang="fr">Ce service trouve, pour une position ou un élément géographique donné, tous les éléments ayant une série d’attributs spécifique qui sont situés à une distance définie par l’utilisateur par rapport à la position ou à l’élément.</skos:scopeNote>
    <skos:prefLabel xml:lang="pt">Serviço de análise de proximidade</skos:prefLabel>
    <skos:scopeNote xml:lang="pt">A partir de uma determinada localização ou elemento geográfico, este serviço encontra todos os objectos com um determinado conjunto de atributos que estão localizados a uma distância definida pelo utilizador relativamente à localização ou ao elemento geográfico.</skos:scopeNote>
    <skos:inScheme rdf:resource="http://inspire.ec.europa.eu/metadata-codelist/SpatialDataServiceCategory" />
    <skos:broader rdf:resource="http://inspire.ec.europa.eu/metadata-codelist/SpatialDataServiceCategory/spatialProcessingService" />
  </skos:Concept>
  <skos:Concept xmlns:skos="http://www.w3.org/2004/02/skos/core#" rdf:about="http://inspire.ec.europa.eu/metadata-codelist/SpatialDataServiceCategory/thematicProcessingService">
    <skos:prefLabel xml:lang="en">Geographic processing services – thematic</skos:prefLabel>
    <skos:prefLabel xml:lang="es">Servicios geográficos de procesamiento de tipo temático</skos:prefLabel>
    <skos:prefLabel xml:lang="fr">Services de traitement géographique — aspects thématiques</skos:prefLabel>
    <skos:prefLabel xml:lang="pt">Serviços de processamento geográfico — elementos temáticos</skos:prefLabel>
    <skos:inScheme rdf:resource="http://inspire.ec.europa.eu/metadata-codelist/SpatialDataServiceCategory" />
    <skos:narrower rdf:resource="http://inspire.ec.europa.eu/metadata-codelist/SpatialDataServiceCategory/thematicGoparameterCalculationService" />
    <skos:narrower rdf:resource="http://inspire.ec.europa.eu/metadata-codelist/SpatialDataServiceCategory/thematicClassificationService" />
    <skos:narrower rdf:resource="http://inspire.ec.europa.eu/metadata-codelist/SpatialDataServiceCategory/thematicFeatureGeneralizationService" />
    <skos:narrower rdf:resource="http://inspire.ec.europa.eu/metadata-codelist/SpatialDataServiceCategory/thematicSubsettingService" />
    <skos:narrower rdf:resource="http://inspire.ec.europa.eu/metadata-codelist/SpatialDataServiceCategory/thematicSpatialCountingService" />
    <skos:narrower rdf:resource="http://inspire.ec.europa.eu/metadata-codelist/SpatialDataServiceCategory/thematicChangeDetectionService" />
    <skos:narrower rdf:resource="http://inspire.ec.europa.eu/metadata-codelist/SpatialDataServiceCategory/thematicGeographicInformationExtractionService" />
    <skos:narrower rdf:resource="http://inspire.ec.europa.eu/metadata-codelist/SpatialDataServiceCategory/thematicImageProcessingService" />
    <skos:narrower rdf:resource="http://inspire.ec.europa.eu/metadata-codelist/SpatialDataServiceCategory/thematicReducedResolutionGenerationService" />
    <skos:narrower rdf:resource="http://inspire.ec.europa.eu/metadata-codelist/SpatialDataServiceCategory/thematicImageManipulationService" />
    <skos:narrower rdf:resource="http://inspire.ec.europa.eu/metadata-codelist/SpatialDataServiceCategory/thematicImageUnderstandingService" />
    <skos:narrower rdf:resource="http://inspire.ec.europa.eu/metadata-codelist/SpatialDataServiceCategory/thematicImageSynthesisService" />
    <skos:narrower rdf:resource="http://inspire.ec.europa.eu/metadata-codelist/SpatialDataServiceCategory/thematicMultibandImageManipulationService" />
    <skos:narrower rdf:resource="http://inspire.ec.europa.eu/metadata-codelist/SpatialDataServiceCategory/thematicObjectDetectionService" />
    <skos:narrower rdf:resource="http://inspire.ec.europa.eu/metadata-codelist/SpatialDataServiceCategory/thematicGeoparsingService" />
    <skos:narrower rdf:resource="http://inspire.ec.europa.eu/metadata-codelist/SpatialDataServiceCategory/thematicGeocodingService" />
  </skos:Concept>
  <skos:Concept xmlns:skos="http://www.w3.org/2004/02/skos/core#" rdf:about="http://inspire.ec.europa.eu/metadata-codelist/SpatialDataServiceCategory/thematicGoparameterCalculationService">
    <skos:prefLabel xml:lang="en">Geoparameter calculation service</skos:prefLabel>
    <skos:scopeNote xml:lang="en">Service to derive application-oriented quantitative results that are not available from the raw data itself.</skos:scopeNote>
    <skos:prefLabel xml:lang="es">Servicio de cálculo de geoparámetros</skos:prefLabel>
    <skos:scopeNote xml:lang="es">Servicio que obtiene resultados cuantitativos orientados a aplicaciones que no están disponibles en los datos brutos en sí.</skos:scopeNote>
    <skos:prefLabel xml:lang="fr">Service de calcul des géoparamètres</skos:prefLabel>
    <skos:scopeNote xml:lang="fr">Service qui dérive des résultats quantitatifs, axés sur les applications, qui ne peuvent pas être obtenus à partir des seules données brutes.</skos:scopeNote>
    <skos:prefLabel xml:lang="pt">Serviço de cálculo de geoparâmetros</skos:prefLabel>
    <skos:scopeNote xml:lang="pt">Serviço que permite obter resultados quantitativos centrados em aplicações que não podem ser obtidos a partir dos próprios dados em bruto.</skos:scopeNote>
    <skos:inScheme rdf:resource="http://inspire.ec.europa.eu/metadata-codelist/SpatialDataServiceCategory" />
    <skos:broader rdf:resource="http://inspire.ec.europa.eu/metadata-codelist/SpatialDataServiceCategory/thematicProcessingService" />
  </skos:Concept>
  <skos:Concept xmlns:skos="http://www.w3.org/2004/02/skos/core#" rdf:about="http://inspire.ec.europa.eu/metadata-codelist/SpatialDataServiceCategory/thematicClassificationService">
    <skos:prefLabel xml:lang="en">Thematic classification service</skos:prefLabel>
    <skos:scopeNote xml:lang="en">Service to classify regions of geographic data based on thematic attributes.</skos:scopeNote>
    <skos:prefLabel xml:lang="es">Servicio de clasificación temática</skos:prefLabel>
    <skos:scopeNote xml:lang="es">Servicio que clasifica regiones de datos geográficos basándose en atributos temáticos.</skos:scopeNote>
    <skos:prefLabel xml:lang="fr">Service de classification thématique</skos:prefLabel>
    <skos:scopeNote xml:lang="fr">Service qui classe des zones de données géographiques sur la base des attributs thématiques.</skos:scopeNote>
    <skos:prefLabel xml:lang="pt">Serviço de classificação temática</skos:prefLabel>
    <skos:scopeNote xml:lang="pt">Serviço que classifica regiões de dados geográficos com base em atributos temáticos.</skos:scopeNote>
    <skos:inScheme rdf:resource="http://inspire.ec.europa.eu/metadata-codelist/SpatialDataServiceCategory" />
    <skos:broader rdf:resource="http://inspire.ec.europa.eu/metadata-codelist/SpatialDataServiceCategory/thematicProcessingService" />
  </skos:Concept>
  <skos:Concept xmlns:skos="http://www.w3.org/2004/02/skos/core#" rdf:about="http://inspire.ec.europa.eu/metadata-codelist/SpatialDataServiceCategory/thematicFeatureGeneralizationService">
    <skos:prefLabel xml:lang="en">Feature generalisation service</skos:prefLabel>
    <skos:scopeNote xml:lang="en">Service that generalises feature types in a feature collection to increase the effectiveness of communication by counteracting the undesirable effects of data reduction.</skos:scopeNote>
    <skos:prefLabel xml:lang="es">Servicio de generalización de fenómenos</skos:prefLabel>
    <skos:scopeNote xml:lang="es">Servicio que generaliza tipos de fenómeno de una colección de fenómenos para aumentar la eficacia de la comunicación contrarrestando los efectos indeseables de la reducción de datos.</skos:scopeNote>
    <skos:prefLabel xml:lang="fr">Service de généralisation d’éléments</skos:prefLabel>
    <skos:scopeNote xml:lang="fr">Service qui généralise les types d’éléments contenus dans une compilation d’éléments afin de renforcer l’efficacité de la communication en remédiant aux effets indésirables de la réduction de données.</skos:scopeNote>
    <skos:prefLabel xml:lang="pt">Serviço de generalização de elementos geográficos</skos:prefLabel>
    <skos:scopeNote xml:lang="pt">Serviço que generaliza os tipos de elementos geográficos numa colecção de elementos geográficos para aumentar a eficácia da comunicação mediante a neutralização dos efeitos indesejáveis da redução de dados.</skos:scopeNote>
    <skos:inScheme rdf:resource="http://inspire.ec.europa.eu/metadata-codelist/SpatialDataServiceCategory" />
    <skos:broader rdf:resource="http://inspire.ec.europa.eu/metadata-codelist/SpatialDataServiceCategory/thematicProcessingService" />
  </skos:Concept>
  <skos:Concept xmlns:skos="http://www.w3.org/2004/02/skos/core#" rdf:about="http://inspire.ec.europa.eu/metadata-codelist/SpatialDataServiceCategory/thematicSubsettingService">
    <skos:prefLabel xml:lang="en">Subsetting service</skos:prefLabel>
    <skos:scopeNote xml:lang="en">Service that extracts data from an input based on parameter values.</skos:scopeNote>
    <skos:prefLabel xml:lang="es">Servicio de subdivisión</skos:prefLabel>
    <skos:scopeNote xml:lang="es">Servicio que extrae datos de entrada basándose en valores de parámetros.</skos:scopeNote>
    <skos:prefLabel xml:lang="fr">Service de définition de sous-ensembles</skos:prefLabel>
    <skos:scopeNote xml:lang="fr">Service permettant d’extraire des données sur la base des paramètres d’entrée.</skos:scopeNote>
    <skos:prefLabel xml:lang="pt">Serviço de definição de subconjuntos</skos:prefLabel>
    <skos:scopeNote xml:lang="pt">Serviço que permite extrair dados a partir de uma fonte baseada em valores de parâmetros.</skos:scopeNote>
    <skos:inScheme rdf:resource="http://inspire.ec.europa.eu/metadata-codelist/SpatialDataServiceCategory" />
    <skos:broader rdf:resource="http://inspire.ec.europa.eu/metadata-codelist/SpatialDataServiceCategory/thematicProcessingService" />
  </skos:Concept>
  <skos:Concept xmlns:skos="http://www.w3.org/2004/02/skos/core#" rdf:about="http://inspire.ec.europa.eu/metadata-codelist/SpatialDataServiceCategory/thematicSpatialCountingService">
    <skos:prefLabel xml:lang="en">Spatial counting service</skos:prefLabel>
    <skos:scopeNote xml:lang="en">Service that counts geographic features.</skos:scopeNote>
    <skos:prefLabel xml:lang="es">Servicio de recuento espacial</skos:prefLabel>
    <skos:scopeNote xml:lang="es">Servicio que cuenta fenómenos geográficos.</skos:scopeNote>
    <skos:prefLabel xml:lang="fr">Service de comptage géographique</skos:prefLabel>
    <skos:scopeNote xml:lang="fr">Service permettant de compter les éléments géographiques.</skos:scopeNote>
    <skos:prefLabel xml:lang="pt">Serviço de contagem geográfica</skos:prefLabel>
    <skos:scopeNote xml:lang="pt">Serviço que permite contar os elementos geográficos.</skos:scopeNote>
    <skos:inScheme rdf:resource="http://inspire.ec.europa.eu/metadata-codelist/SpatialDataServiceCategory" />
    <skos:broader rdf:resource="http://inspire.ec.europa.eu/metadata-codelist/SpatialDataServiceCategory/thematicProcessingService" />
  </skos:Concept>
  <skos:Concept xmlns:skos="http://www.w3.org/2004/02/skos/core#" rdf:about="http://inspire.ec.europa.eu/metadata-codelist/SpatialDataServiceCategory/thematicChangeDetectionService">
    <skos:prefLabel xml:lang="en">Change detection service</skos:prefLabel>
    <skos:scopeNote xml:lang="en">Service to find differences between two data sets that represent the same geographical area at different times.</skos:scopeNote>
    <skos:prefLabel xml:lang="es">Servicio de detección de cambios</skos:prefLabel>
    <skos:scopeNote xml:lang="es">Servicio que encuentra las diferencias entre dos conjuntos de datos que representan la misma zona geográfica en diferentes momentos.</skos:scopeNote>
    <skos:prefLabel xml:lang="fr">Service de détection des changements</skos:prefLabel>
    <skos:scopeNote xml:lang="fr">Service permettant de déceler les différences entre deux séries de données qui représentent la même zone géographique à des moments différents.</skos:scopeNote>
    <skos:prefLabel xml:lang="pt">Serviço de detecção de alterações</skos:prefLabel>
    <skos:scopeNote xml:lang="pt">Serviço que permite encontrar diferenças entre dois conjuntos de dados que representam a mesma zona geográfica em momentos diferentes.</skos:scopeNote>
    <skos:inScheme rdf:resource="http://inspire.ec.europa.eu/metadata-codelist/SpatialDataServiceCategory" />
    <skos:broader rdf:resource="http://inspire.ec.europa.eu/metadata-codelist/SpatialDataServiceCategory/thematicProcessingService" />
  </skos:Concept>
  <skos:Concept xmlns:skos="http://www.w3.org/2004/02/skos/core#" rdf:about="http://inspire.ec.europa.eu/metadata-codelist/SpatialDataServiceCategory/thematicGeographicInformationExtractionService">
    <skos:prefLabel xml:lang="en">Geographic information extraction services</skos:prefLabel>
    <skos:scopeNote xml:lang="en">Services supporting the extraction of feature and terrain information from remotely sensed and scanned images.</skos:scopeNote>
    <skos:prefLabel xml:lang="es">Servicios de extracción de información geográfica</skos:prefLabel>
    <skos:scopeNote xml:lang="es">Servicios que soportan la extracción de información sobre fenómenos y sobre el terreno a partir de imágenes capturadas por teledetección e imágenes escaneadas.</skos:scopeNote>
    <skos:prefLabel xml:lang="fr">Services d’extraction d’informations géographiques</skos:prefLabel>
    <skos:scopeNote xml:lang="fr">Services permettant l’extraction d’informations sur les éléments et le terrain à partir d’images de télédétection et d’images scannées.</skos:scopeNote>
    <skos:prefLabel xml:lang="pt">Serviços de extracção de informação geográfica</skos:prefLabel>
    <skos:scopeNote xml:lang="pt">Serviços que permitem a extracção de elementos geográficos e de informações sobre o terreno a partir de imagens rasterizadas ou provenientes de sensores remotos.</skos:scopeNote>
    <skos:inScheme rdf:resource="http://inspire.ec.europa.eu/metadata-codelist/SpatialDataServiceCategory" />
    <skos:broader rdf:resource="http://inspire.ec.europa.eu/metadata-codelist/SpatialDataServiceCategory/thematicProcessingService" />
  </skos:Concept>
  <skos:Concept xmlns:skos="http://www.w3.org/2004/02/skos/core#" rdf:about="http://inspire.ec.europa.eu/metadata-codelist/SpatialDataServiceCategory/thematicImageProcessingService">
    <skos:prefLabel xml:lang="en">Image processing service</skos:prefLabel>
    <skos:scopeNote xml:lang="en">Service to change the values of thematic attributes of an image using a mathematical function.</skos:scopeNote>
    <skos:prefLabel xml:lang="es">Servicio de procesamiento de imágenes</skos:prefLabel>
    <skos:scopeNote xml:lang="es">Servicio que cambia los valores de los atributos temáticos de una imagen usando una función matemática.</skos:scopeNote>
    <skos:prefLabel xml:lang="fr">Service de traitement d’images</skos:prefLabel>
    <skos:scopeNote xml:lang="fr">Service permettant de modifier les valeurs des attributs thématiques d’une image au moyen d’une fonction mathématique.</skos:scopeNote>
    <skos:prefLabel xml:lang="pt">Serviço de processamento de imagens</skos:prefLabel>
    <skos:scopeNote xml:lang="pt">Serviço que permite modificar os valores dos atributos temáticos de uma imagem utilizando uma função matemática.</skos:scopeNote>
    <skos:inScheme rdf:resource="http://inspire.ec.europa.eu/metadata-codelist/SpatialDataServiceCategory" />
    <skos:broader rdf:resource="http://inspire.ec.europa.eu/metadata-codelist/SpatialDataServiceCategory/thematicProcessingService" />
  </skos:Concept>
  <skos:Concept xmlns:skos="http://www.w3.org/2004/02/skos/core#" rdf:about="http://inspire.ec.europa.eu/metadata-codelist/SpatialDataServiceCategory/thematicReducedResolutionGenerationService">
    <skos:prefLabel xml:lang="en">Reduced resolution generation service</skos:prefLabel>
    <skos:scopeNote xml:lang="en">Service that reduces the resolution of an image.</skos:scopeNote>
    <skos:prefLabel xml:lang="es">Servicio de generación de resolución reducida</skos:prefLabel>
    <skos:scopeNote xml:lang="es">Servicio que reduce la resolución de una imagen.</skos:scopeNote>
    <skos:prefLabel xml:lang="fr">Service de réduction de la résolution</skos:prefLabel>
    <skos:scopeNote xml:lang="fr">Service permettant de réduire la résolution d’une image.</skos:scopeNote>
    <skos:prefLabel xml:lang="pt">Serviço de redução de resolução</skos:prefLabel>
    <skos:scopeNote xml:lang="pt">Serviço que permite diminuir a resolução de uma imagem.</skos:scopeNote>
    <skos:inScheme rdf:resource="http://inspire.ec.europa.eu/metadata-codelist/SpatialDataServiceCategory" />
    <skos:broader rdf:resource="http://inspire.ec.europa.eu/metadata-codelist/SpatialDataServiceCategory/thematicProcessingService" />
  </skos:Concept>
  <skos:Concept xmlns:skos="http://www.w3.org/2004/02/skos/core#" rdf:about="http://inspire.ec.europa.eu/metadata-codelist/SpatialDataServiceCategory/thematicImageManipulationService">
    <skos:prefLabel xml:lang="en">Image Manipulation Services</skos:prefLabel>
    <skos:scopeNote xml:lang="en">Services for manipulating data values in images: changing colour and contrast values, applying various filters, manipulating image resolution, noise removal, "striping", systematic-radiometric corrections, atmospheric attenuation, changes in scene illumination, etc.</skos:scopeNote>
    <skos:prefLabel xml:lang="es">Servicio de manipulación de imágenes</skos:prefLabel>
    <skos:scopeNote xml:lang="es">Servicio para la manipulación de los valores de datos en una imagen: cambio de valores de color y contraste, aplicación de filtros diversos, manipulación de la resolución de imágenes, eliminación de ruidos, eliminación del "efecto de bandeado"(striping), aplicación de correcciones radiométricas sistemáticas, atenuación atmosférica, cambios en la iluminación de la escena, etc.</skos:scopeNote>
    <skos:prefLabel xml:lang="fr">Services de manipulation d’images</skos:prefLabel>
    <skos:scopeNote xml:lang="fr">Services permettant de manipuler les valeurs des données dans les images: modification des valeurs de couleur et de contraste, application de différents filtres, manipulation de la résolution de l’image, réduction du bruit, réduction des stries, corrections radiométriques, atténuation atmosphérique, changement d’illumination de la scène, etc.</skos:scopeNote>
    <skos:prefLabel xml:lang="pt">Serviços de manipulação de imagens</skos:prefLabel>
    <skos:scopeNote xml:lang="pt">Serviços que permitem manipular os dados das imagens: modificação dos valores de cor e contraste, aplicação de vários filtros, manipulação da resolução da imagem, eliminação de ruído, eliminação do efeito de "striping", correcções radiométricas sistemáticas, atenuação atmosférica, modificações na iluminação da imagem, etc.</skos:scopeNote>
    <skos:inScheme rdf:resource="http://inspire.ec.europa.eu/metadata-codelist/SpatialDataServiceCategory" />
    <skos:broader rdf:resource="http://inspire.ec.europa.eu/metadata-codelist/SpatialDataServiceCategory/thematicProcessingService" />
  </skos:Concept>
  <skos:Concept xmlns:skos="http://www.w3.org/2004/02/skos/core#" rdf:about="http://inspire.ec.europa.eu/metadata-codelist/SpatialDataServiceCategory/thematicImageUnderstandingService">
    <skos:prefLabel xml:lang="en">Image understanding services</skos:prefLabel>
    <skos:scopeNote xml:lang="en">Services that provide automated image change detection, registered image differencing, significance-of-difference analysis and display, and area-based and model-based differencing.</skos:scopeNote>
    <skos:prefLabel xml:lang="es">Servicio de comprensión de imágenes</skos:prefLabel>
    <skos:scopeNote xml:lang="es">Servicio que proporcionan detección automática de cambios de imagen, registro de diferencias en la imagen, análisis y visualización de diferencias significativas, y diferenciación basada en superficies y en modelos.</skos:scopeNote>
    <skos:prefLabel xml:lang="fr">Services de compréhension d’images</skos:prefLabel>
    <skos:scopeNote xml:lang="fr">Services permettant la détection automatisée des changements d’images, la différenciation des images rectifiées, l’analyse et l’affichage de l’importance des différences, et la différenciation par zone et par modèle.</skos:scopeNote>
    <skos:prefLabel xml:lang="pt">Serviços de compreensão de imagens</skos:prefLabel>
    <skos:scopeNote xml:lang="pt">Serviços que permitem a detecção automática de alterações entre imagens, o cálculo de diferenças entre imagens co-registadas, a análise e visualização da significância estatística da diferença entre imagens e o cálculo de diferenças entre imagens baseado em áreas e modelos.</skos:scopeNote>
    <skos:inScheme rdf:resource="http://inspire.ec.europa.eu/metadata-codelist/SpatialDataServiceCategory" />
    <skos:broader rdf:resource="http://inspire.ec.europa.eu/metadata-codelist/SpatialDataServiceCategory/thematicProcessingService" />
  </skos:Concept>
  <skos:Concept xmlns:skos="http://www.w3.org/2004/02/skos/core#" rdf:about="http://inspire.ec.europa.eu/metadata-codelist/SpatialDataServiceCategory/thematicImageSynthesisService">
    <skos:prefLabel xml:lang="en">Image synthesis services</skos:prefLabel>
    <skos:scopeNote xml:lang="en">Services for creating or transforming images using computer-based spatial models, perspective transformations, and manipulations of image characteristics to improve visibility, sharpen resolution, and/or reduce the effects of cloud cover or haze.</skos:scopeNote>
    <skos:prefLabel xml:lang="es">Servicio de síntesis de imágenes</skos:prefLabel>
    <skos:scopeNote xml:lang="es">Servicio de creación y transformación de imágenes que utiliza modelos espaciales automatizados, transformaciones de perspectiva, y manipulaciones de características de la imagen para mejorar la visibilidad, afinar la resolución o reducir los efectos de coberturas nubosas y neblinas.</skos:scopeNote>
    <skos:prefLabel xml:lang="fr">Services de synthèse d’images</skos:prefLabel>
    <skos:scopeNote xml:lang="fr">Services permettant de créer ou de transformer des images au moyen de modèles spatiaux informatisés, de transformations de perspective, et de manipulations de caractéristiques de l’image en vue d’améliorer la visibilité et la résolution et/ou de réduire les effets de la couverture nuageuse ou de la brume.</skos:scopeNote>
    <skos:prefLabel xml:lang="pt">Serviços de síntese de imagens</skos:prefLabel>
    <skos:scopeNote xml:lang="pt">Serviços que permitem criar ou transformar imagens utilizando modelos espaciais em computador, transformações de perspectiva e manipulações de características da imagem para melhorar a sua visualização e resolução e/ou reduzir os efeitos da cobertura de nuvens ou da neblina.</skos:scopeNote>
    <skos:inScheme rdf:resource="http://inspire.ec.europa.eu/metadata-codelist/SpatialDataServiceCategory" />
    <skos:broader rdf:resource="http://inspire.ec.europa.eu/metadata-codelist/SpatialDataServiceCategory/thematicProcessingService" />
  </skos:Concept>
  <skos:Concept xmlns:skos="http://www.w3.org/2004/02/skos/core#" rdf:about="http://inspire.ec.europa.eu/metadata-codelist/SpatialDataServiceCategory/thematicMultibandImageManipulationService">
    <skos:prefLabel xml:lang="en">Multiband image manipulation</skos:prefLabel>
    <skos:scopeNote xml:lang="en">Services that modify an image using the multiple bands of the image.</skos:scopeNote>
    <skos:prefLabel xml:lang="es">Manipulación de imágenes multibanda</skos:prefLabel>
    <skos:scopeNote xml:lang="es">Servicio que modifica una imagen usando sus múltiples bandas.</skos:scopeNote>
    <skos:prefLabel xml:lang="fr">Manipulation d’images multibandes</skos:prefLabel>
    <skos:scopeNote xml:lang="fr">Services permettant de modifier une image en utilisant les différentes bandes spectrales de l’image.</skos:scopeNote>
    <skos:prefLabel xml:lang="pt">Serviços de manipulação de imagens multibandas</skos:prefLabel>
    <skos:scopeNote xml:lang="pt">Serviços que permitem modificar uma imagem utilizando as suas várias bandas.</skos:scopeNote>
    <skos:inScheme rdf:resource="http://inspire.ec.europa.eu/metadata-codelist/SpatialDataServiceCategory" />
    <skos:broader rdf:resource="http://inspire.ec.europa.eu/metadata-codelist/SpatialDataServiceCategory/thematicProcessingService" />
  </skos:Concept>
  <skos:Concept xmlns:skos="http://www.w3.org/2004/02/skos/core#" rdf:about="http://inspire.ec.europa.eu/metadata-codelist/SpatialDataServiceCategory/thematicObjectDetectionService">
    <skos:prefLabel xml:lang="en">Object detection service</skos:prefLabel>
    <skos:scopeNote xml:lang="en">Service to detect real-world objects in an image.</skos:scopeNote>
    <skos:prefLabel xml:lang="es">Servicio de detección de objetos</skos:prefLabel>
    <skos:scopeNote xml:lang="es">Servicio que detecta objetos del mundo real en una imagen.</skos:scopeNote>
    <skos:prefLabel xml:lang="fr">Service de détection d’objets</skos:prefLabel>
    <skos:scopeNote xml:lang="fr">Service permettant de détecter les objets du monde réel dans une image.</skos:scopeNote>
    <skos:prefLabel xml:lang="pt">Serviço de detecção de objectos</skos:prefLabel>
    <skos:scopeNote xml:lang="pt">Serviço que permite identificar objectos do mundo real numa imagem.</skos:scopeNote>
    <skos:inScheme rdf:resource="http://inspire.ec.europa.eu/metadata-codelist/SpatialDataServiceCategory" />
    <skos:broader rdf:resource="http://inspire.ec.europa.eu/metadata-codelist/SpatialDataServiceCategory/thematicProcessingService" />
  </skos:Concept>
  <skos:Concept xmlns:skos="http://www.w3.org/2004/02/skos/core#" rdf:about="http://inspire.ec.europa.eu/metadata-codelist/SpatialDataServiceCategory/thematicGeoparsingService">
    <skos:prefLabel xml:lang="en">Geoparsing service</skos:prefLabel>
    <skos:scopeNote xml:lang="en">Service to scan text documents for location-based references, such as a place names, addresses, postal codes, etc., in preparation for passage to a geocoding service.</skos:scopeNote>
    <skos:prefLabel xml:lang="es">Servicio de geoanálisis sintáctico</skos:prefLabel>
    <skos:scopeNote xml:lang="es">Servicio que escanea documentos de texto para encontrar referencias basadas en la localización, por ejemplo, topónimos, direcciones, códigos postales, etc., como preparación para pasar a un servicio de geocodificación.</skos:scopeNote>
    <skos:prefLabel xml:lang="fr">Service d’analyse géosémantique</skos:prefLabel>
    <skos:scopeNote xml:lang="fr">Service permettant de rechercher dans les documents textuels les références à des lieux, comme les toponymes, les adresses, les codes postaux, etc., dans la perspective d’un service de géocodage.</skos:scopeNote>
    <skos:prefLabel xml:lang="pt">Serviço de geoidentificação</skos:prefLabel>
    <skos:scopeNote xml:lang="pt">Serviço que permite procurar em documentos textuais referências a locais, como topónimos, endereços, códigos postais, etc., para fins de preparação da passagem para um serviço de geocodificação.</skos:scopeNote>
    <skos:inScheme rdf:resource="http://inspire.ec.europa.eu/metadata-codelist/SpatialDataServiceCategory" />
    <skos:broader rdf:resource="http://inspire.ec.europa.eu/metadata-codelist/SpatialDataServiceCategory/thematicProcessingService" />
  </skos:Concept>
  <skos:Concept xmlns:skos="http://www.w3.org/2004/02/skos/core#" rdf:about="http://inspire.ec.europa.eu/metadata-codelist/SpatialDataServiceCategory/thematicGeocodingService">
    <skos:prefLabel xml:lang="en">Geocoding service</skos:prefLabel>
    <skos:scopeNote xml:lang="en">Service to augment location-based text references with geographic coordinates (or some other spatial reference).</skos:scopeNote>
    <skos:prefLabel xml:lang="es">Servicio de geocodificación</skos:prefLabel>
    <skos:scopeNote xml:lang="es">Servicio que mejora las referencias textuales basadas en la localización con coordenadas geográficas (o a alguna otra referencia espacial).</skos:scopeNote>
    <skos:prefLabel xml:lang="fr">Service de géocodage</skos:prefLabel>
    <skos:scopeNote xml:lang="fr">Service permettant, dans les textes, de compléter les références à des lieux en indiquant les coordonnées géographiques (ou une autre référence spatiale).</skos:scopeNote>
    <skos:prefLabel xml:lang="pt">Serviço de geocodificação</skos:prefLabel>
    <skos:scopeNote xml:lang="pt">Serviço que permite complementar referências textuais baseadas na localização com coordenadas geográficas (ou outra referência espacial).</skos:scopeNote>
    <skos:inScheme rdf:resource="http://inspire.ec.europa.eu/metadata-codelist/SpatialDataServiceCategory" />
    <skos:broader rdf:resource="http://inspire.ec.europa.eu/metadata-codelist/SpatialDataServiceCategory/thematicProcessingService" />
  </skos:Concept>
  <skos:Concept xmlns:skos="http://www.w3.org/2004/02/skos/core#" rdf:about="http://inspire.ec.europa.eu/metadata-codelist/SpatialDataServiceCategory/temporalProcessingService">
    <skos:prefLabel xml:lang="en">Geographic processing services – temporal</skos:prefLabel>
    <skos:prefLabel xml:lang="es">Servicios geográficos de procesamiento de tipo temporal</skos:prefLabel>
    <skos:prefLabel xml:lang="fr">Services de traitement géographique — aspects temporels</skos:prefLabel>
    <skos:prefLabel xml:lang="pt">Serviços de processamento geográfico — elementos temporais</skos:prefLabel>
    <skos:inScheme rdf:resource="http://inspire.ec.europa.eu/metadata-codelist/SpatialDataServiceCategory" />
    <skos:narrower rdf:resource="http://inspire.ec.europa.eu/metadata-codelist/SpatialDataServiceCategory/temporalReferenceSystemTransformationService" />
    <skos:narrower rdf:resource="http://inspire.ec.europa.eu/metadata-codelist/SpatialDataServiceCategory/temporalSubsettingService" />
    <skos:narrower rdf:resource="http://inspire.ec.europa.eu/metadata-codelist/SpatialDataServiceCategory/temporalSamplingService" />
    <skos:narrower rdf:resource="http://inspire.ec.europa.eu/metadata-codelist/SpatialDataServiceCategory/temporalProximityAnalysisService" />
  </skos:Concept>
  <skos:Concept xmlns:skos="http://www.w3.org/2004/02/skos/core#" rdf:about="http://inspire.ec.europa.eu/metadata-codelist/SpatialDataServiceCategory/temporalReferenceSystemTransformationService">
    <skos:prefLabel xml:lang="en">Temporal reference system transformation service</skos:prefLabel>
    <skos:scopeNote xml:lang="en">Service to change the values of temporal instances from one temporal reference system to another temporal reference system.</skos:scopeNote>
    <skos:prefLabel xml:lang="es">Servicio de transformación de sistemas de referencia temporal</skos:prefLabel>
    <skos:scopeNote xml:lang="es">Servicio que cambia los valores de las instancias temporales de un sistema de referencia temporal a otro.</skos:scopeNote>
    <skos:prefLabel xml:lang="fr">Service de transformation du système de référence temporel</skos:prefLabel>
    <skos:scopeNote xml:lang="fr">Service permettant de modifier les valeurs des occurrences temporelles d’un système de référence temporelle à un autre système de référence temporelle.</skos:scopeNote>
    <skos:prefLabel xml:lang="pt">Serviço de transformação do sistema de referência temporal</skos:prefLabel>
    <skos:scopeNote xml:lang="pt">Serviço que permite modificar os valores das ocorrências temporais de um sistema de referência temporal para outro sistema de referência temporal.</skos:scopeNote>
    <skos:inScheme rdf:resource="http://inspire.ec.europa.eu/metadata-codelist/SpatialDataServiceCategory" />
    <skos:broader rdf:resource="http://inspire.ec.europa.eu/metadata-codelist/SpatialDataServiceCategory/temporalProcessingService" />
  </skos:Concept>
  <skos:Concept xmlns:skos="http://www.w3.org/2004/02/skos/core#" rdf:about="http://inspire.ec.europa.eu/metadata-codelist/SpatialDataServiceCategory/temporalSubsettingService">
    <skos:prefLabel xml:lang="en">Subsetting service</skos:prefLabel>
    <skos:scopeNote xml:lang="en">Service that extracts data from an input in a continuous interval based on temporal position values.</skos:scopeNote>
    <skos:prefLabel xml:lang="es">Servicio de subdivisión</skos:prefLabel>
    <skos:scopeNote xml:lang="es">Servicio que extrae datos de una entrada en un intervalo continuo basándose en valores de posición temporal.</skos:scopeNote>
    <skos:prefLabel xml:lang="fr">Service de définition de sous-ensembles</skos:prefLabel>
    <skos:scopeNote xml:lang="fr">Service permettant d’extraire des données dans un intervalle continu sur la base de valeurs de position temporelle.</skos:scopeNote>
    <skos:prefLabel xml:lang="pt">Serviço de definição de subconjuntos</skos:prefLabel>
    <skos:scopeNote xml:lang="pt">Serviço que permite extrair dados de uma fonte num intervalo contínuo com base em valores de posição temporal.</skos:scopeNote>
    <skos:inScheme rdf:resource="http://inspire.ec.europa.eu/metadata-codelist/SpatialDataServiceCategory" />
    <skos:broader rdf:resource="http://inspire.ec.europa.eu/metadata-codelist/SpatialDataServiceCategory/temporalProcessingService" />
  </skos:Concept>
  <skos:Concept xmlns:skos="http://www.w3.org/2004/02/skos/core#" rdf:about="http://inspire.ec.europa.eu/metadata-codelist/SpatialDataServiceCategory/temporalSamplingService">
    <skos:prefLabel xml:lang="en">Sampling service</skos:prefLabel>
    <skos:scopeNote xml:lang="en">Service that extracts data from an input using a consistent sampling scheme based on temporal position values.</skos:scopeNote>
    <skos:prefLabel xml:lang="es">Servicio de muestreo</skos:prefLabel>
    <skos:scopeNote xml:lang="es">Servicio que extrae datos de una entrada usando un esquemade muestreo coherente basado en valores de posición temporal.</skos:scopeNote>
    <skos:prefLabel xml:lang="fr">Service d’échantillonnage</skos:prefLabel>
    <skos:scopeNote xml:lang="fr">Service permettant d’extraire des données au moyen d’un système d’échantillonnage cohérent sur la base des valeurs de position temporelle.</skos:scopeNote>
    <skos:prefLabel xml:lang="pt">Serviço de amostragem</skos:prefLabel>
    <skos:scopeNote xml:lang="pt">Serviço que permite extrair dados de uma fonte por meio de um sistema de amostragem coerente baseado em valores de localização temporal.</skos:scopeNote>
    <skos:inScheme rdf:resource="http://inspire.ec.europa.eu/metadata-codelist/SpatialDataServiceCategory" />
    <skos:broader rdf:resource="http://inspire.ec.europa.eu/metadata-codelist/SpatialDataServiceCategory/temporalProcessingService" />
  </skos:Concept>
  <skos:Concept xmlns:skos="http://www.w3.org/2004/02/skos/core#" rdf:about="http://inspire.ec.europa.eu/metadata-codelist/SpatialDataServiceCategory/temporalProximityAnalysisService">
    <skos:prefLabel xml:lang="en">Temporal proximity analysis service</skos:prefLabel>
    <skos:scopeNote xml:lang="en">Given a temporal interval or event, find all objects with a given set of attributes that are located within a user-specified interval from the interval or event.</skos:scopeNote>
    <skos:prefLabel xml:lang="es">Servicio de análisis de proximidad temporal</skos:prefLabel>
    <skos:scopeNote xml:lang="es">Dado un intervalo temporal o un evento, este servicio encuentra todos los objetos con un conjunto dado de atributos que están localizados dentro de un intervalo temporal, especificado por el usuario, con respecto al intervalo o evento dado.</skos:scopeNote>
    <skos:prefLabel xml:lang="fr">Service d’analyse de proximité</skos:prefLabel>
    <skos:scopeNote xml:lang="fr">Ce service trouve, pour un intervalle temporel ou un événement donné, tous les objets ayant une série d’attributs spécifique qui sont situés dans un intervalle défini par l’utilisateur par rapport à l’intervalle ou à l’élément.</skos:scopeNote>
    <skos:prefLabel xml:lang="pt">Serviço de análise de proximidade temporal</skos:prefLabel>
    <skos:scopeNote xml:lang="pt">A partir de um determinado intervalo de tempo ou evento, este serviço encontra todos os objectos com um determinado conjunto de atributos que estão localizados dentro de um intervalo definido pelo utilizador em relação ao referido intervalo ou evento.</skos:scopeNote>
    <skos:inScheme rdf:resource="http://inspire.ec.europa.eu/metadata-codelist/SpatialDataServiceCategory" />
    <skos:broader rdf:resource="http://inspire.ec.europa.eu/metadata-codelist/SpatialDataServiceCategory/temporalProcessingService" />
  </skos:Concept>
  <skos:Concept xmlns:skos="http://www.w3.org/2004/02/skos/core#" rdf:about="http://inspire.ec.europa.eu/metadata-codelist/SpatialDataServiceCategory/metadataProcessingService">
    <skos:prefLabel xml:lang="en">Geographic processing services – metadata</skos:prefLabel>
    <skos:prefLabel xml:lang="es">Servicios geográficos de procesamiento de tipo metadatos</skos:prefLabel>
    <skos:prefLabel xml:lang="fr">Services de traitement géographique — métadonnées</skos:prefLabel>
    <skos:prefLabel xml:lang="pt">Serviços de processamento geográfico – metadados</skos:prefLabel>
    <skos:inScheme rdf:resource="http://inspire.ec.europa.eu/metadata-codelist/SpatialDataServiceCategory" />
    <skos:narrower rdf:resource="http://inspire.ec.europa.eu/metadata-codelist/SpatialDataServiceCategory/metadataStatisticalCalculationService" />
    <skos:narrower rdf:resource="http://inspire.ec.europa.eu/metadata-codelist/SpatialDataServiceCategory/metadataGeographicAnnotationService" />
  </skos:Concept>
  <skos:Concept xmlns:skos="http://www.w3.org/2004/02/skos/core#" rdf:about="http://inspire.ec.europa.eu/metadata-codelist/SpatialDataServiceCategory/metadataStatisticalCalculationService">
    <skos:prefLabel xml:lang="en">Statistical calculation service</skos:prefLabel>
    <skos:scopeNote xml:lang="en">Service to calculate the statistics of a data set.</skos:scopeNote>
    <skos:prefLabel xml:lang="es">Servicio de cálculo estadístico</skos:prefLabel>
    <skos:scopeNote xml:lang="es">Servicio que calcula las estadísticas de un conjunto de datos.</skos:scopeNote>
    <skos:prefLabel xml:lang="fr">Service de calcul statistique</skos:prefLabel>
    <skos:scopeNote xml:lang="fr">Service permettant de calculer les statistiques d’un ensemble de données.</skos:scopeNote>
    <skos:prefLabel xml:lang="pt">Serviço de cálculo estatístico</skos:prefLabel>
    <skos:scopeNote xml:lang="pt">Serviço que permite calcular as estatísticas de um conjunto de dados.</skos:scopeNote>
    <skos:inScheme rdf:resource="http://inspire.ec.europa.eu/metadata-codelist/SpatialDataServiceCategory" />
    <skos:broader rdf:resource="http://inspire.ec.europa.eu/metadata-codelist/SpatialDataServiceCategory/metadataProcessingService" />
  </skos:Concept>
  <skos:Concept xmlns:skos="http://www.w3.org/2004/02/skos/core#" rdf:about="http://inspire.ec.europa.eu/metadata-codelist/SpatialDataServiceCategory/metadataGeographicAnnotationService">
    <skos:prefLabel xml:lang="en">Geographic annotation services</skos:prefLabel>
    <skos:scopeNote xml:lang="en">Services to add ancillary information to an image or a feature in a feature collection.</skos:scopeNote>
    <skos:prefLabel xml:lang="es">Servicios geográficos de anotación</skos:prefLabel>
    <skos:scopeNote xml:lang="es">Servicios que añaden información complementaria a una imagen o fenómeno de una colección de fenómenos.</skos:scopeNote>
    <skos:prefLabel xml:lang="fr">Services d’annotation géographique</skos:prefLabel>
    <skos:scopeNote xml:lang="fr">Services permettant d’ajouter des informations complémentaires à une image ou un élément dans une compilation d’éléments.</skos:scopeNote>
    <skos:prefLabel xml:lang="pt">Serviços de anotação geográfica</skos:prefLabel>
    <skos:scopeNote xml:lang="pt">Serviços que permitem acrescentar informação auxiliar a uma imagem ou elemento geográfico numa colecção de elementos geográficos.</skos:scopeNote>
    <skos:inScheme rdf:resource="http://inspire.ec.europa.eu/metadata-codelist/SpatialDataServiceCategory" />
    <skos:broader rdf:resource="http://inspire.ec.europa.eu/metadata-codelist/SpatialDataServiceCategory/metadataProcessingService" />
  </skos:Concept>
  <skos:Concept xmlns:skos="http://www.w3.org/2004/02/skos/core#" rdf:about="http://inspire.ec.europa.eu/metadata-codelist/SpatialDataServiceCategory/comService">
    <skos:prefLabel xml:lang="en">Geographic communication services</skos:prefLabel>
    <skos:prefLabel xml:lang="es">Servicios geográficos de comunicación</skos:prefLabel>
    <skos:prefLabel xml:lang="fr">Services de communication géographique</skos:prefLabel>
    <skos:prefLabel xml:lang="pt">Serviços de comunicação geográfica</skos:prefLabel>
    <skos:inScheme rdf:resource="http://inspire.ec.europa.eu/metadata-codelist/SpatialDataServiceCategory" />
    <skos:narrower rdf:resource="http://inspire.ec.europa.eu/metadata-codelist/SpatialDataServiceCategory/comEncodingService" />
    <skos:narrower rdf:resource="http://inspire.ec.europa.eu/metadata-codelist/SpatialDataServiceCategory/comTransferService" />
    <skos:narrower rdf:resource="http://inspire.ec.europa.eu/metadata-codelist/SpatialDataServiceCategory/comGeographicCompressionService" />
    <skos:narrower rdf:resource="http://inspire.ec.europa.eu/metadata-codelist/SpatialDataServiceCategory/comGeographicFormatConversionService" />
    <skos:narrower rdf:resource="http://inspire.ec.europa.eu/metadata-codelist/SpatialDataServiceCategory/comMessagingService" />
    <skos:narrower rdf:resource="http://inspire.ec.europa.eu/metadata-codelist/SpatialDataServiceCategory/comRemoteFileAndExecutableManagement" />
  </skos:Concept>
  <skos:Concept xmlns:skos="http://www.w3.org/2004/02/skos/core#" rdf:about="http://inspire.ec.europa.eu/metadata-codelist/SpatialDataServiceCategory/comEncodingService">
    <skos:prefLabel xml:lang="en">Encoding service</skos:prefLabel>
    <skos:scopeNote xml:lang="en">Service that provides implementation of an encoding rule and provides an interface to encoding and decoding functionality.</skos:scopeNote>
    <skos:prefLabel xml:lang="es">Servicio de codificación</skos:prefLabel>
    <skos:scopeNote xml:lang="es">Servicio que permite la implementación de una regla de codificación y proporciona una interfaz con la función de codificación y decodificación.</skos:scopeNote>
    <skos:prefLabel xml:lang="fr">Service d’encodage</skos:prefLabel>
    <skos:scopeNote xml:lang="fr">Service permettant la mise en œuvre d’une règle d’encodage et servant d’interface pour la fonctionnalité d’encodage et de décodage.</skos:scopeNote>
    <skos:prefLabel xml:lang="pt">Serviço de codificação</skos:prefLabel>
    <skos:scopeNote xml:lang="pt">Serviço que permite a execução de uma regra de codificação e proporciona uma interface para a funcionalidade de codificação e de descodificação.</skos:scopeNote>
    <skos:inScheme rdf:resource="http://inspire.ec.europa.eu/metadata-codelist/SpatialDataServiceCategory" />
    <skos:broader rdf:resource="http://inspire.ec.europa.eu/metadata-codelist/SpatialDataServiceCategory/comService" />
  </skos:Concept>
  <skos:Concept xmlns:skos="http://www.w3.org/2004/02/skos/core#" rdf:about="http://inspire.ec.europa.eu/metadata-codelist/SpatialDataServiceCategory/comTransferService">
    <skos:prefLabel xml:lang="en">Transfer service</skos:prefLabel>
    <skos:scopeNote xml:lang="en">Service that provides implementation of one or more transfer protocols, which allows data transfer between distributed information systems over offline or online communication media.</skos:scopeNote>
    <skos:prefLabel xml:lang="es">Servicio de transferencia</skos:prefLabel>
    <skos:scopeNote xml:lang="es">Servicio que permite la implementación de uno o más protocolos de transferencia que permiten la transferencia de datos entre sistemas de información distribuidos por medios de comunicación en línea o fuera de línea.</skos:scopeNote>
    <skos:prefLabel xml:lang="fr">Service de transfert</skos:prefLabel>
    <skos:scopeNote xml:lang="fr">Service permettant la mise en œuvre d’un ou plusieurs protocoles de transfert, ce qui permet le transfert de données entre des systèmes d’information distribués via des moyens de communication hors ligne ou en ligne.</skos:scopeNote>
    <skos:prefLabel xml:lang="pt">Serviço de transferência</skos:prefLabel>
    <skos:scopeNote xml:lang="pt">Serviço que permite executar um ou mais protocolos de transferência, a fim de transferir dados entre sistemas de informação distribuídos através de meios de comunicação fora de linha ou em linha.</skos:scopeNote>
    <skos:inScheme rdf:resource="http://inspire.ec.europa.eu/metadata-codelist/SpatialDataServiceCategory" />
    <skos:broader rdf:resource="http://inspire.ec.europa.eu/metadata-codelist/SpatialDataServiceCategory/comService" />
  </skos:Concept>
  <skos:Concept xmlns:skos="http://www.w3.org/2004/02/skos/core#" rdf:about="http://inspire.ec.europa.eu/metadata-codelist/SpatialDataServiceCategory/comGeographicCompressionService">
    <skos:prefLabel xml:lang="en">Geographic compression service</skos:prefLabel>
    <skos:scopeNote xml:lang="en">Service that converts spatial portions of a feature collection to and from compressed form.</skos:scopeNote>
    <skos:prefLabel xml:lang="es">Servicio de compresión de datos geográficos</skos:prefLabel>
    <skos:scopeNote xml:lang="es">Servicio que comprime o descomprime porciones espaciales de una colección de fenómenos.</skos:scopeNote>
    <skos:prefLabel xml:lang="fr">Service de compression géographique</skos:prefLabel>
    <skos:scopeNote xml:lang="fr">Service permettant de convertir les parties spatiales d’une compilation d’éléments pour les faire passer de la forme non compressée à la forme compressée, et vice versa.</skos:scopeNote>
    <skos:prefLabel xml:lang="pt">Serviço de compressão geográfica</skos:prefLabel>
    <skos:scopeNote xml:lang="pt">Serviço que permite converter partes espaciais de uma colecção de elementos geográficos para formato comprimido, e vice-versa.</skos:scopeNote>
    <skos:inScheme rdf:resource="http://inspire.ec.europa.eu/metadata-codelist/SpatialDataServiceCategory" />
    <skos:broader rdf:resource="http://inspire.ec.europa.eu/metadata-codelist/SpatialDataServiceCategory/comService" />
  </skos:Concept>
  <skos:Concept xmlns:skos="http://www.w3.org/2004/02/skos/core#" rdf:about="http://inspire.ec.europa.eu/metadata-codelist/SpatialDataServiceCategory/comGeographicFormatConversionService">
    <skos:prefLabel xml:lang="en">Geographic format conversion service</skos:prefLabel>
    <skos:scopeNote xml:lang="en">Service that converts from one geographic data format to another.</skos:scopeNote>
    <skos:prefLabel xml:lang="es">Servicio de conversión de formato de datos geográficos</skos:prefLabel>
    <skos:scopeNote xml:lang="es">Servicio que convierte datos geográficos de un formato a otro.</skos:scopeNote>
    <skos:prefLabel xml:lang="fr">Service de conversion de format géographique</skos:prefLabel>
    <skos:scopeNote xml:lang="fr">Service permettant de passer d’un format de données géographiques à un autre.</skos:scopeNote>
    <skos:prefLabel xml:lang="pt">Serviço de conversão de formato geográfico</skos:prefLabel>
    <skos:scopeNote xml:lang="pt">Serviço que permite a conversão de um formato de dados geográficos para outro.</skos:scopeNote>
    <skos:inScheme rdf:resource="http://inspire.ec.europa.eu/metadata-codelist/SpatialDataServiceCategory" />
    <skos:broader rdf:resource="http://inspire.ec.europa.eu/metadata-codelist/SpatialDataServiceCategory/comService" />
  </skos:Concept>
  <skos:Concept xmlns:skos="http://www.w3.org/2004/02/skos/core#" rdf:about="http://inspire.ec.europa.eu/metadata-codelist/SpatialDataServiceCategory/comMessagingService">
    <skos:prefLabel xml:lang="en">Messaging service</skos:prefLabel>
    <skos:scopeNote xml:lang="en">Service that allows multiple users to simultaneously view, comment about, and request edits of feature collections.</skos:scopeNote>
    <skos:prefLabel xml:lang="es">Servicio de mensajería</skos:prefLabel>
    <skos:scopeNote xml:lang="es">Servicio que permite a múltiples usuarios ver simultáneamente colecciones de fenómenos, así como comentarlas y solicitar su edición.</skos:scopeNote>
    <skos:prefLabel xml:lang="fr">Service de messagerie</skos:prefLabel>
    <skos:scopeNote xml:lang="fr">Service permettant simultanément à plusieurs utilisateurs de visualiser et de commenter des compilations d’éléments et d’en demander des révisions.</skos:scopeNote>
    <skos:prefLabel xml:lang="pt">Serviço de transmissão de mensagens</skos:prefLabel>
    <skos:scopeNote xml:lang="pt">Serviço que permite simultaneamente a vários utilizadores visualizar e comentar colecções de elementos geográficos e solicitar revisões das mesmas.</skos:scopeNote>
    <skos:inScheme rdf:resource="http://inspire.ec.europa.eu/metadata-codelist/SpatialDataServiceCategory" />
    <skos:broader rdf:resource="http://inspire.ec.europa.eu/metadata-codelist/SpatialDataServiceCategory/comService" />
  </skos:Concept>
  <skos:Concept xmlns:skos="http://www.w3.org/2004/02/skos/core#" rdf:about="http://inspire.ec.europa.eu/metadata-codelist/SpatialDataServiceCategory/comRemoteFileAndExecutableManagement">
    <skos:prefLabel xml:lang="en">Remote file and executable management</skos:prefLabel>
    <skos:scopeNote xml:lang="en">Service that provides access to secondary storage of geographic features as if it were local to the client.</skos:scopeNote>
    <skos:prefLabel xml:lang="es">Gestión de ejecutables y ficheros remotos</skos:prefLabel>
    <skos:scopeNote xml:lang="es">Servicio que proporciona acceso a un almacenamiento secundario de fenómenos geográficos como si fuera local para el cliente.</skos:scopeNote>
    <skos:prefLabel xml:lang="fr">Gestion des fichiers éloignés et des fichiers exécutables</skos:prefLabel>
    <skos:scopeNote xml:lang="fr">Service permettant d’accéder à un stockage distant des éléments géographiques comme s’il s’agissait de ressources locales.</skos:scopeNote>
    <skos:prefLabel xml:lang="pt">Gestão remota de ficheiros e de executáveis</skos:prefLabel>
    <skos:scopeNote xml:lang="pt">Serviço que permite o acesso a um sistema secundário de armazenamento de elementos geográficos como se este fosse um recurso local do cliente.</skos:scopeNote>
    <skos:inScheme rdf:resource="http://inspire.ec.europa.eu/metadata-codelist/SpatialDataServiceCategory" />
    <skos:broader rdf:resource="http://inspire.ec.europa.eu/metadata-codelist/SpatialDataServiceCategory/comService" />
  </skos:Concept>
</rdf:RDF>

